change to circuit, scheduling oracle and proof adjusting

model/agp32UpdateLib.sml
@@ -13,37 +13,37 @@ val  clist_update_state_tac =
   qpat_abbrev_tac `s3 = ForwardW _ _ _` >>
   fs [Once procs_def] >>
   qpat_abbrev_tac `s4 = IF_instr_update _ _ _` >>
+  fs [Once procs_def] >>
+  qpat_abbrev_tac `s5 = WB_update _ _ _` >>
   fs [Once procs_def] >>  
-  qpat_abbrev_tac `s5 = ID_opc_func_update _ _ _` >>
+  qpat_abbrev_tac `s6 = ID_opc_func_update _ _ _` >>
   fs [Once procs_def] >>
-  qpat_abbrev_tac `s6 = ID_imm_update _ _ _` >>
+  qpat_abbrev_tac `s7 = ID_imm_update _ _ _` >>
   fs [Once procs_def] >>
-  qpat_abbrev_tac `s7 = ID_data_update _ _ _` >>
+  qpat_abbrev_tac `s8 = ID_data_update _ _ _` >>
   fs [Once procs_def] >>
-  qpat_abbrev_tac `s8 = EX_ctrl_update _ _ _` >>
+  qpat_abbrev_tac `s9 = MEM_imm_update _ _ _` >>
   fs [Once procs_def] >>
-  qpat_abbrev_tac `s9 = EX_forward_data _ _ _` >>
+  qpat_abbrev_tac `s10 = EX_ctrl_update _ _ _` >>
   fs [Once procs_def] >>
-  qpat_abbrev_tac `s10 = EX_ALU_input_update _ _ _` >>
+  qpat_abbrev_tac `s11 = EX_forward_data _ _ _` >>
   fs [Once procs_def] >>
-  qpat_abbrev_tac `s11 = EX_compute_enable_update _ _ _` >>
+  qpat_abbrev_tac `s12 = EX_ALU_input_update _ _ _` >>
   fs [Once procs_def] >>
-  qpat_abbrev_tac `s12 = EX_ALU_update _ _ _` >>
+  qpat_abbrev_tac `s13 = EX_compute_enable_update _ _ _` >>
   fs [Once procs_def] >>
-  qpat_abbrev_tac `s13 = EX_SHIFT_update _ _ _` >>
+  qpat_abbrev_tac `s14 = EX_ALU_update _ _ _` >>
   fs [Once procs_def] >>
-  qpat_abbrev_tac `s14 = EX_jump_sel_addr_update _ _ _` >>
+  qpat_abbrev_tac `s15 = EX_SHIFT_update _ _ _` >>
   fs [Once procs_def] >>
-  qpat_abbrev_tac `s15 = EX_data_rec_update _ _ _` >>
+  qpat_abbrev_tac `s16 = EX_jump_sel_addr_update _ _ _` >>
   fs [Once procs_def] >>
-  qpat_abbrev_tac `s16 = IF_PC_input_update _ _ _` >>
+  qpat_abbrev_tac `s17 = EX_data_rec_update _ _ _` >>
   fs [Once procs_def] >>
-  qpat_abbrev_tac `s17 = MEM_ctrl_update _ _ _` >>
+  qpat_abbrev_tac `s18 = IF_PC_input_update _ _ _` >>
   fs [Once procs_def] >>
-  qpat_abbrev_tac `s18 = MEM_imm_update _ _ _` >>
+  qpat_abbrev_tac `s19 = MEM_ctrl_update _ _ _` >>
   fs [procs_def] >>
-  qpat_abbrev_tac `s19 = WB_update _ _ _` >>
-  fs [Once procs_def] >>
   qpat_abbrev_tac `s20 = Hazard_ctrl _ _ _`);
 
 val clist_update_state_before_ALU_tac =
@@ -58,19 +58,23 @@ val clist_update_state_before_ALU_tac =
   rw [Once procs_def] >>
   qpat_abbrev_tac `s4 = IF_instr_update _ _ _` >>
   rw [Once procs_def] >>
-  qpat_abbrev_tac `s5 = ID_opc_func_update _ _ _` >>
+  qpat_abbrev_tac `s5 = WB_update _ _ _` >>
   rw [Once procs_def] >>
-  qpat_abbrev_tac `s6 = ID_imm_update _ _ _` >>
+  qpat_abbrev_tac `s6 = ID_opc_func_update _ _ _` >>
   rw [Once procs_def] >>
-  qpat_abbrev_tac `s7 = ID_data_update _ _ _` >>
+  qpat_abbrev_tac `s7 = ID_imm_update _ _ _` >>
   rw [Once procs_def] >>
-  qpat_abbrev_tac `s8 = EX_ctrl_update _ _ _` >>
+  qpat_abbrev_tac `s8 = ID_data_update _ _ _` >>
   rw [Once procs_def] >>
-  qpat_abbrev_tac `s9 = EX_forward_data _ _ _` >>
+  qpat_abbrev_tac `s9 = MEM_imm_update _ _ _` >>
   rw [Once procs_def] >>
-  qpat_abbrev_tac `s10 = EX_ALU_input_update _ _ _` >>
+  qpat_abbrev_tac `s10 = EX_ctrl_update _ _ _` >>
+  rw [Once procs_def] >>
+  qpat_abbrev_tac `s11 = EX_forward_data _ _ _` >>
+  rw [Once procs_def] >>
+  qpat_abbrev_tac `s12 = EX_ALU_input_update _ _ _` >>
   rw [procs_def] >>
-  qpat_abbrev_tac `s11 = EX_compute_enable_update _ _ _`);
+  qpat_abbrev_tac `s13 = EX_compute_enable_update _ _ _`);
 
 val slist_update_state_tac =
  (rw [Once procs_def] >>
