proof/agp32InternalScript.sml
@@ -65,7 +65,7 @@ Proof
   rw [] >> Q.ABBREV_TAC `s = agp32 fext fbits t` >>
   Q.ABBREV_TAC `s' = procs [agp32_next_state; WB_pipeline; MEM_pipeline; EX_pipeline;
                             REG_write; ID_pipeline; IF_PC_update; Acc_compute] (fext t) s s` >>
-  Q.ABBREV_TAC `s'' = procs [ForwardA; ForwardB; ForwardW; IF_instr_update;
+  Q.ABBREV_TAC `s'' = procs [ForwardA; ForwardB; ForwardW; IF_instr_update; WB_update;
                              ID_opc_func_update; ID_imm_update] (fext (SUC t)) s' s'` >>
   `((agp32 fext fbits (SUC t)).ID.ID_addrA_disable <=>
   (ID_data_update (fext (SUC t)) s' s'').ID.ID_addrA_disable) /\
@@ -84,7 +84,7 @@ Proof
   rw [] >> Q.ABBREV_TAC `s = agp32 fext fbits t` >>
   Q.ABBREV_TAC `s' = procs [agp32_next_state; WB_pipeline; MEM_pipeline; EX_pipeline;
                             REG_write; ID_pipeline; IF_PC_update; Acc_compute] (fext t) s s` >>
-  Q.ABBREV_TAC `s'' = procs [ForwardA; ForwardB; ForwardW; IF_instr_update;
+  Q.ABBREV_TAC `s'' = procs [ForwardA; ForwardB; ForwardW; IF_instr_update; WB_update;
                              ID_opc_func_update; ID_imm_update] (fext (SUC t)) s' s'` >>
   `((agp32 fext fbits (SUC t)).ID.ID_addrB_disable <=>
   (ID_data_update (fext (SUC t)) s' s'').ID.ID_addrB_disable) /\
@@ -103,7 +103,7 @@ Proof
   rw [] >> Q.ABBREV_TAC `s = agp32 fext fbits t` >>
   Q.ABBREV_TAC `s' = procs [agp32_next_state; WB_pipeline; MEM_pipeline; EX_pipeline;
                             REG_write; ID_pipeline; IF_PC_update; Acc_compute] (fext t) s s` >>
-  Q.ABBREV_TAC `s'' = procs [ForwardA; ForwardB; ForwardW; IF_instr_update;
+  Q.ABBREV_TAC `s'' = procs [ForwardA; ForwardB; ForwardW; IF_instr_update; WB_update;
                              ID_opc_func_update; ID_imm_update] (fext (SUC t)) s' s'` >>
   `((agp32 fext fbits (SUC t)).ID.ID_addrW_disable <=>
   (ID_data_update (fext (SUC t)) s' s'').ID.ID_addrW_disable) /\
@@ -113,6 +113,139 @@ Proof
            agp32_ID_imm_data_updated_by_ID_data_update,agp32_ID_data_updated_by_ID_data_update] >>
   fs [ID_data_update_def,MUX_21_def]
 QED
+
+(** relation between ID addr_disable data_updated and data singals **)
+Theorem agp32_ID_addrA_enable_dataA_read_dataA_updated:
+  !fext fbits t.
+    ~(agp32 fext fbits (SUC t)).ID.ID_addrA_disable ==>
+    (agp32 fext fbits (SUC t)).ID.ID_dataA = (agp32 fext fbits (SUC t)).ID.ID_read_dataA_updated
+Proof
+  rw [] >> Q.ABBREV_TAC `s = agp32 fext fbits t` >>
+  Q.ABBREV_TAC `s' = procs [agp32_next_state; WB_pipeline; MEM_pipeline; EX_pipeline;
+                            REG_write; ID_pipeline; IF_PC_update; Acc_compute] (fext t) s s` >>
+  Q.ABBREV_TAC `s'' = procs [ForwardA; ForwardB; ForwardW; IF_instr_update; WB_update;
+                             ID_opc_func_update; ID_imm_update] (fext (SUC t)) s' s'` >>
+  `((agp32 fext fbits (SUC t)).ID.ID_addrA_disable <=>
+    (ID_data_update (fext (SUC t)) s' s'').ID.ID_addrA_disable) /\
+  ((agp32 fext fbits (SUC t)).ID.ID_read_dataA_updated =
+   (ID_data_update (fext (SUC t)) s' s'').ID.ID_read_dataA_updated) /\
+  ((agp32 fext fbits (SUC t)).ID.ID_dataA = (ID_data_update (fext (SUC t)) s' s'').ID.ID_dataA)`
+    by fs [Abbr `s`,Abbr `s'`,Abbr `s''`,agp32_ID_flag_updated_by_ID_data_update,
+           agp32_ID_read_data_updated_updated_by_ID_data_update,
+           agp32_ID_data_updated_by_ID_data_update] >>
+  fs [ID_data_update_def,MUX_21_def]
+QED
+
+Theorem agp32_ID_addrB_enable_dataB_read_dataB_updated:
+  !fext fbits t.
+    ~(agp32 fext fbits (SUC t)).ID.ID_addrB_disable ==>
+    (agp32 fext fbits (SUC t)).ID.ID_dataB = (agp32 fext fbits (SUC t)).ID.ID_read_dataB_updated
+Proof
+  rw [] >> Q.ABBREV_TAC `s = agp32 fext fbits t` >>
+  Q.ABBREV_TAC `s' = procs [agp32_next_state; WB_pipeline; MEM_pipeline; EX_pipeline;
+                            REG_write; ID_pipeline; IF_PC_update; Acc_compute] (fext t) s s` >>
+  Q.ABBREV_TAC `s'' = procs [ForwardA; ForwardB; ForwardW; IF_instr_update; WB_update;
+                             ID_opc_func_update; ID_imm_update] (fext (SUC t)) s' s'` >>
+  `((agp32 fext fbits (SUC t)).ID.ID_addrB_disable <=>
+    (ID_data_update (fext (SUC t)) s' s'').ID.ID_addrB_disable) /\
+  ((agp32 fext fbits (SUC t)).ID.ID_read_dataB_updated =
+   (ID_data_update (fext (SUC t)) s' s'').ID.ID_read_dataB_updated) /\
+  ((agp32 fext fbits (SUC t)).ID.ID_dataB = (ID_data_update (fext (SUC t)) s' s'').ID.ID_dataB)`
+    by fs [Abbr `s`,Abbr `s'`,Abbr `s''`,agp32_ID_flag_updated_by_ID_data_update,
+           agp32_ID_read_data_updated_updated_by_ID_data_update,
+           agp32_ID_data_updated_by_ID_data_update] >>
+  fs [ID_data_update_def,MUX_21_def]
+QED
+
+Theorem agp32_ID_addrW_enable_dataW_read_dataW_updated:
+  !fext fbits t.
+    ~(agp32 fext fbits (SUC t)).ID.ID_addrW_disable ==>
+    (agp32 fext fbits (SUC t)).ID.ID_dataW = (agp32 fext fbits (SUC t)).ID.ID_read_dataW_updated
+Proof
+  rw [] >> Q.ABBREV_TAC `s = agp32 fext fbits t` >>
+  Q.ABBREV_TAC `s' = procs [agp32_next_state; WB_pipeline; MEM_pipeline; EX_pipeline;
+                            REG_write; ID_pipeline; IF_PC_update; Acc_compute] (fext t) s s` >>
+  Q.ABBREV_TAC `s'' = procs [ForwardA; ForwardB; ForwardW; IF_instr_update; WB_update;
+                             ID_opc_func_update; ID_imm_update] (fext (SUC t)) s' s'` >>
+  `((agp32 fext fbits (SUC t)).ID.ID_addrW_disable <=>
+    (ID_data_update (fext (SUC t)) s' s'').ID.ID_addrW_disable) /\
+  ((agp32 fext fbits (SUC t)).ID.ID_read_dataW_updated =
+   (ID_data_update (fext (SUC t)) s' s'').ID.ID_read_dataW_updated) /\
+  ((agp32 fext fbits (SUC t)).ID.ID_dataW = (ID_data_update (fext (SUC t)) s' s'').ID.ID_dataW)`
+    by fs [Abbr `s`,Abbr `s'`,Abbr `s''`,agp32_ID_flag_updated_by_ID_data_update,
+           agp32_ID_read_data_updated_updated_by_ID_data_update,
+           agp32_ID_data_updated_by_ID_data_update] >>
+  fs [ID_data_update_def,MUX_21_def]
+QED
+
+
+(** relation between ID Forward flags, read_data and read_data_updated **)
+Theorem agp32_ID_not_ForwardA_read_dataA_read_dataA_updated:
+  !fext fbits t.
+    ~(agp32 fext fbits (SUC t)).ID.ID_ForwardA ==>
+    (agp32 fext fbits (SUC t)).ID.ID_read_dataA_updated = (agp32 fext fbits (SUC t)).ID.ID_read_dataA
+Proof
+  rw [] >> Q.ABBREV_TAC `s = agp32 fext fbits t` >>
+  Q.ABBREV_TAC `s' = procs [agp32_next_state; WB_pipeline; MEM_pipeline; EX_pipeline;
+                            REG_write; ID_pipeline; IF_PC_update; Acc_compute] (fext t) s s` >>
+  Q.ABBREV_TAC `s'' = procs [ForwardA; ForwardB; ForwardW; IF_instr_update; WB_update;
+                             ID_opc_func_update; ID_imm_update] (fext (SUC t)) s' s'` >>
+  `((agp32 fext fbits (SUC t)).ID.ID_ForwardA <=>
+    (ID_data_update (fext (SUC t)) s' s'').ID.ID_ForwardA) /\
+  ((agp32 fext fbits (SUC t)).ID.ID_read_dataA_updated =
+   (ID_data_update (fext (SUC t)) s' s'').ID.ID_read_dataA_updated) /\
+  ((agp32 fext fbits (SUC t)).ID.ID_read_dataA =
+   (ID_data_update (fext (SUC t)) s' s'').ID.ID_read_dataA)`
+    by fs [Abbr `s`,Abbr `s'`,Abbr `s''`,agp32_ID_Forward_flags_updated_by_ID_data_update,
+           agp32_ID_read_data_updated_by_ID_data_update,
+           agp32_ID_read_data_updated_updated_by_ID_data_update] >>
+  fs [ID_data_update_def,MUX_21_def] >> METIS_TAC []
+QED
+
+Theorem agp32_ID_not_ForwardB_read_dataB_read_dataB_updated:
+  !fext fbits t.
+    ~(agp32 fext fbits (SUC t)).ID.ID_ForwardB ==>
+    (agp32 fext fbits (SUC t)).ID.ID_read_dataB_updated = (agp32 fext fbits (SUC t)).ID.ID_read_dataB
+Proof
+  rw [] >> Q.ABBREV_TAC `s = agp32 fext fbits t` >>
+  Q.ABBREV_TAC `s' = procs [agp32_next_state; WB_pipeline; MEM_pipeline; EX_pipeline;
+                            REG_write; ID_pipeline; IF_PC_update; Acc_compute] (fext t) s s` >>
+  Q.ABBREV_TAC `s'' = procs [ForwardA; ForwardB; ForwardW; IF_instr_update; WB_update;
+                             ID_opc_func_update; ID_imm_update] (fext (SUC t)) s' s'` >>
+  `((agp32 fext fbits (SUC t)).ID.ID_ForwardB <=>
+    (ID_data_update (fext (SUC t)) s' s'').ID.ID_ForwardB) /\
+  ((agp32 fext fbits (SUC t)).ID.ID_read_dataB_updated =
+   (ID_data_update (fext (SUC t)) s' s'').ID.ID_read_dataB_updated) /\
+  ((agp32 fext fbits (SUC t)).ID.ID_read_dataB =
+   (ID_data_update (fext (SUC t)) s' s'').ID.ID_read_dataB)`
+    by fs [Abbr `s`,Abbr `s'`,Abbr `s''`,agp32_ID_Forward_flags_updated_by_ID_data_update,
+           agp32_ID_read_data_updated_by_ID_data_update,
+           agp32_ID_read_data_updated_updated_by_ID_data_update] >>
+  fs [ID_data_update_def,MUX_21_def] >> METIS_TAC []
+QED
+
+Theorem agp32_ID_not_ForwardW_read_dataW_read_dataW_updated:
+  !fext fbits t.
+    ~(agp32 fext fbits (SUC t)).ID.ID_ForwardW ==>
+    (agp32 fext fbits (SUC t)).ID.ID_read_dataW_updated = (agp32 fext fbits (SUC t)).ID.ID_read_dataW
+Proof
+  rw [] >> Q.ABBREV_TAC `s = agp32 fext fbits t` >>
+  Q.ABBREV_TAC `s' = procs [agp32_next_state; WB_pipeline; MEM_pipeline; EX_pipeline;
+                            REG_write; ID_pipeline; IF_PC_update; Acc_compute] (fext t) s s` >>
+  Q.ABBREV_TAC `s'' = procs [ForwardA; ForwardB; ForwardW; IF_instr_update; WB_update;
+                             ID_opc_func_update; ID_imm_update] (fext (SUC t)) s' s'` >>
+  `((agp32 fext fbits (SUC t)).ID.ID_ForwardW <=>
+    (ID_data_update (fext (SUC t)) s' s'').ID.ID_ForwardW) /\
+  ((agp32 fext fbits (SUC t)).ID.ID_read_dataW_updated =
+   (ID_data_update (fext (SUC t)) s' s'').ID.ID_read_dataW_updated) /\
+  ((agp32 fext fbits (SUC t)).ID.ID_read_dataW =
+   (ID_data_update (fext (SUC t)) s' s'').ID.ID_read_dataW)`
+    by fs [Abbr `s`,Abbr `s'`,Abbr `s''`,agp32_ID_Forward_flags_updated_by_ID_data_update,
+           agp32_ID_read_data_updated_by_ID_data_update,
+           agp32_ID_read_data_updated_updated_by_ID_data_update] >>
+  fs [ID_data_update_def,MUX_21_def] >> METIS_TAC []
+QED
+
 
 (** EX stage **)
 Theorem agp32_EX_opc_implies_EX_func:
@@ -381,15 +514,10 @@ QED
 Theorem agp32_ID_EX_write_enable_no_MEM_stg_op:
   !fext fbits t.
     (agp32 fext fbits t).ID.ID_EX_write_enable ==>
-    ((agp32 fext fbits t).MEM.MEM_opc <> 2w) /\
-    ((agp32 fext fbits t).MEM.MEM_opc <> 3w) /\
-    ((agp32 fext fbits t).MEM.MEM_opc <> 4w) /\
-    ((agp32 fext fbits t).MEM.MEM_opc <> 5w) /\
-    ((agp32 fext fbits t).MEM.MEM_opc <> 8w) /\
-    ((agp32 fext fbits t).MEM.MEM_opc <> 12w)
+    ~isMemOp_hw_op (agp32 fext fbits t)
 Proof
-  rpt gen_tac >> rpt disch_tac >> Cases_on `t` >>
-  fs [agp32_def,mk_module_def,mk_circuit_def] >-
+  rw [] >> Cases_on `t` >>
+  fs [agp32_def,mk_module_def,mk_circuit_def,isMemOp_hw_op_def] >-
    (clist_update_state_tac >>
     fs [Abbr `s20`,Hazard_ctrl_def] >>
     Cases_on `s19.state = 1w \/ s19.state = 2w \/ s19.state = 3w \/
@@ -443,6 +571,14 @@ Proof
       ForwardA_unchanged_MEM_pipeline_items]
 QED
 
+Theorem MEM_stg_op_agp32_ID_EX_write_disable:
+  !fext fbits t.
+    isMemOp_hw_op (agp32 fext fbits t) ==>
+    ~(agp32 fext fbits t).ID.ID_EX_write_enable
+Proof
+  rw [] >> METIS_TAC [agp32_ID_EX_write_enable_no_MEM_stg_op]
+QED
+
 (* MEM_state_flag *)
 (** MEM_state_flag and WB_state_flag **)
 Theorem agp32_MEM_state_flag_eq_WB_state_flag:
@@ -464,6 +600,68 @@ Proof
   Cases_on `s'.EX.EX_jump_sel` >> fs []
 QED
 
+(** ID_EX_write_enable, MEM_state_flag and MEM_opc **)
+Theorem agp32_ID_EX_write_disable_MEM_state_enable_MEM_stg_op:
+  !fext fbits t.
+    ~(agp32 fext fbits t).ID.ID_EX_write_enable ==>
+    (agp32 fext fbits t).MEM.MEM_state_flag ==>
+    isMemOp_hw_op (agp32 fext fbits t)
+Proof
+  rw [] >> Cases_on `t` >>
+  fs [agp32_def,mk_module_def,mk_circuit_def,isMemOp_hw_op_def] >-
+   (clist_update_state_tac >>
+    fs [Abbr `s20`,Hazard_ctrl_def] >>
+    Cases_on `s19.state = 1w \/ s19.state = 2w \/ s19.state = 3w \/
+              s19.state = 4w \/ s19.state = 5w \/ s19.state = 6w` >> fs [] >>
+    Cases_on `(fext 0).ready` >> fs [] >>
+    Cases_on `(agp32_init fbits).MEM.MEM_opc = 2w \/ (agp32_init fbits).MEM.MEM_opc = 3w \/
+              (agp32_init fbits).MEM.MEM_opc = 4w \/ (agp32_init fbits).MEM.MEM_opc = 5w \/      
+              (agp32_init fbits).MEM.MEM_opc = 8w \/ (agp32_init fbits).MEM.MEM_opc = 12w` >> fs [] >>
+    Cases_on `s19.EX.EX_jump_sel` >> fs [] >>
+    fs [Abbr `s19`,Abbr `s18`,Abbr `s17`,Abbr `s16`,Abbr `s15`,Abbr `s14`,
+        Abbr `s13`,Abbr `s12`,Abbr `s11`,Abbr `s10`,Abbr `s9`,Abbr `s8`,Abbr `s7`,
+        Abbr `s6`,Abbr `s5`,Abbr `s4`,Abbr `s3`,Abbr `s2`,Abbr `s1`,
+        WB_update_unchanged_MEM_pipeline_items,
+        MEM_imm_update_unchanged_MEM_pipeline_items,MEM_ctrl_update_unchanged_MEM_pipeline_items,
+        EX_data_rec_update_unchanged_MEM_pipeline_items,
+        EX_jump_sel_addr_update_unchanged_MEM_pipeline_items,
+        EX_SHIFT_update_unchanged_MEM_pipeline_items,EX_ALU_update_unchanged_MEM_pipeline_items,
+        EX_compute_enable_update_unchanged_MEM_pipeline_items,
+        EX_ALU_input_update_unchanged_MEM_pipeline_items,
+        EX_forward_data_unchanged_MEM_pipeline_items,EX_ctrl_update_unchanged_MEM_pipeline_items,
+        ID_data_update_unchanged_MEM_pipeline_items,ID_imm_update_unchanged_MEM_pipeline_items,
+        ID_opc_func_update_unchanged_MEM_pipeline_items,
+        IF_PC_input_update_unchanged_MEM_pipeline_items,IF_instr_update_def,
+        ForwardW_unchanged_MEM_pipeline_items,ForwardB_unchanged_MEM_pipeline_items,
+        ForwardA_unchanged_MEM_pipeline_items]) >>
+  qpat_abbrev_tac `s' = mk_circuit (procs _) (procs _) (agp32_init fbits) fext t` >>
+  qpat_abbrev_tac `s'' = procs _ (fext t) s' s'` >>
+  clist_update_state_tac >>
+  fs [Abbr `s20`,Hazard_ctrl_def] >>
+  Cases_on `s19.state = 1w \/ s19.state = 2w \/ s19.state = 3w \/
+            s19.state = 4w \/ s19.state = 5w \/ s19.state = 6w` >> fs [] >> fs [] >>
+  Cases_on `(fext (SUC n)).ready` >> fs [] >>
+  Cases_on `s''.MEM.MEM_opc = 2w \/ s''.MEM.MEM_opc = 3w \/ s''.MEM.MEM_opc = 4w \/
+            s''.MEM.MEM_opc = 8w \/ s''.MEM.MEM_opc = 5w \/ s''.MEM.MEM_opc = 12w` >> fs [] >> fs [] >>
+  Cases_on `s19.EX.EX_jump_sel` >> fs [] >>
+  fs [Abbr `s19`,Abbr `s18`,Abbr `s17`,Abbr `s16`,Abbr `s15`,Abbr `s14`,
+      Abbr `s13`,Abbr `s12`,Abbr `s11`,Abbr `s10`,Abbr `s9`,Abbr `s8`,Abbr `s7`,
+      Abbr `s6`,Abbr `s5`,Abbr `s4`,Abbr `s3`,Abbr `s2`,Abbr `s1`,
+      WB_update_unchanged_MEM_pipeline_items,
+      MEM_imm_update_unchanged_MEM_pipeline_items,MEM_ctrl_update_unchanged_MEM_pipeline_items,
+      EX_data_rec_update_unchanged_MEM_pipeline_items,
+      EX_jump_sel_addr_update_unchanged_MEM_pipeline_items,
+      EX_SHIFT_update_unchanged_MEM_pipeline_items,EX_ALU_update_unchanged_MEM_pipeline_items,
+      EX_compute_enable_update_unchanged_MEM_pipeline_items,
+      EX_ALU_input_update_unchanged_MEM_pipeline_items,
+      EX_forward_data_unchanged_MEM_pipeline_items,EX_ctrl_update_unchanged_MEM_pipeline_items,
+      ID_data_update_unchanged_MEM_pipeline_items,ID_imm_update_unchanged_MEM_pipeline_items,
+      ID_opc_func_update_unchanged_MEM_pipeline_items,
+      IF_PC_input_update_unchanged_MEM_pipeline_items,IF_instr_update_def,
+      ForwardW_unchanged_MEM_pipeline_items,ForwardB_unchanged_MEM_pipeline_items,
+      ForwardA_unchanged_MEM_pipeline_items]
+QED
+
 
 (* initial values *)
 (** initial EX_PC_sel = 0w **)
@@ -474,21 +672,23 @@ Proof
   rw [agp32_def,mk_module_def,mk_circuit_def] >>
   clist_update_state_tac >>
   fs [Abbr `s20`,Abbr `s19`,Abbr `s18`,Abbr `s17`,Abbr `s16`,Abbr `s15`,
-      Abbr `s14`,Abbr `s13`,Abbr `s12`,Abbr `s11`,Abbr `s10`,Abbr `s9`,Abbr `s8`,
-      Hazard_ctrl_unchanged_EX_ctrl_items,WB_update_unchanged_EX_ctrl_items,
-      MEM_imm_update_unchanged_EX_ctrl_items,MEM_ctrl_update_unchanged_EX_ctrl_items,
+      Abbr `s14`,Abbr `s13`,Abbr `s12`,Abbr `s11`,Abbr `s10`,
+      Hazard_ctrl_unchanged_EX_ctrl_items,
+      MEM_ctrl_update_unchanged_EX_ctrl_items,
       IF_PC_input_update_def,EX_data_rec_update_unchanged_EX_ctrl_items,
       EX_jump_sel_addr_update_unchanged_EX_ctrl_items,
       EX_SHIFT_update_unchanged_EX_ctrl_items,EX_ALU_update_unchanged_EX_ctrl_items,
       EX_compute_enable_update_unchanged_EX_ctrl_items,
       EX_ALU_input_update_unchanged_EX_ctrl_items,
       EX_forward_data_unchanged_EX_ctrl_items] >>
-  Cases_on `s7.ID.ID_EX_write_enable` >-
+  Cases_on `s9.ID.ID_EX_write_enable` >-
    fs [EX_ctrl_update_def,agp32_init_def] >>
   rw [EX_ctrl_update_def] >>      
-  fs [Abbr `s7`,Abbr `s6`,Abbr `s5`,Abbr `s4`,Abbr `s3`,Abbr `s2`,Abbr `s1`,
+  fs [Abbr `s9`,Abbr `s8`,Abbr `s7`,Abbr `s6`,Abbr `s5`,Abbr `s4`,Abbr `s3`,Abbr `s2`,Abbr `s1`,
+      MEM_imm_update_unchanged_EX_ctrl_items,
       ID_data_update_unchanged_EX_ctrl_items,ID_imm_update_unchanged_EX_ctrl_items,
-      ID_opc_func_update_unchanged_EX_ctrl_items,IF_instr_update_def,
+      ID_opc_func_update_unchanged_EX_ctrl_items,
+      WB_update_unchanged_EX_ctrl_items,IF_instr_update_def,
       ForwardA_def,ForwardB_def,ForwardW_def] >>
    rw [agp32_init_def]
 QED
@@ -501,10 +701,8 @@ Proof
   rw [] >> `(agp32 fext fbits 0).EX.EX_PC_sel = 0w` by rw [agp32_init_EX_PC_sel] >>
   fs [agp32_def,mk_module_def,mk_circuit_def] >>
   clist_update_state_tac >>
-  fs [Abbr `s20`,Abbr `s19`,Abbr `s18`,Abbr `s17`,Abbr `s16`,Abbr `s15`,Abbr `s14`,
+  fs [Abbr `s20`,Abbr `s19`,Abbr `s18`,Abbr `s17`,Abbr `s16`,
       Hazard_ctrl_unchanged_EX_jump,Hazard_ctrl_unchanged_EX_ctrl_items,
-      WB_update_unchanged_EX_jump,WB_update_unchanged_EX_ctrl_items,
-      MEM_imm_update_unchanged_EX_jump,MEM_imm_update_unchanged_EX_ctrl_items,
       MEM_ctrl_update_unchanged_EX_jump,MEM_ctrl_update_unchanged_EX_ctrl_items,
       IF_PC_input_update_def,EX_data_rec_update_unchanged_EX_jump,
       EX_data_rec_update_unchanged_EX_ctrl_items,
@@ -520,14 +718,15 @@ Proof
   rw [] >> `~(agp32 fext fbits 0).EX.EX_jump_sel` by rw [agp32_init_EX_jump_sel] >>
   fs [agp32_def,mk_module_def,mk_circuit_def] >>
   clist_update_state_tac >>
-  fs [Abbr `s20`,Abbr `s19`,Abbr `s18`,Abbr `s17`,Abbr `s16`,
+  fs [Abbr `s20`,Abbr `s19`,Abbr `s18`,
       Hazard_ctrl_unchanged_IF,Hazard_ctrl_unchanged_EX_jump,
-      WB_update_unchanged_IF,WB_update_unchanged_EX_jump,
-      MEM_imm_update_unchanged_IF,MEM_imm_update_unchanged_EX_jump,
       MEM_ctrl_update_unchanged_IF,MEM_ctrl_update_unchanged_EX_jump] >>
   fs [IF_PC_input_update_def,MUX_21_def] >>
-  fs [Abbr `s15`,Abbr `s14`,Abbr `s13`,Abbr `s12`,Abbr `s11`,Abbr `s10`,Abbr `s9`,
-      Abbr `s8`,Abbr `s7`,Abbr `s6`,Abbr `s5`,Abbr `s4`,Abbr `s3`,Abbr `s2`,Abbr `s1`,
+  fs [Abbr `s17`,Abbr `s16`,Abbr `s15`,Abbr `s14`,Abbr `s13`,
+      Abbr `s12`,Abbr `s11`,Abbr `s10`,Abbr `s9`,Abbr `s8`,
+      Abbr `s7`,Abbr `s6`,Abbr `s5`,Abbr `s4`,Abbr `s3`,Abbr `s2`,Abbr `s1`,
+      WB_update_unchanged_IF,WB_update_unchanged_EX_jump,
+      MEM_imm_update_unchanged_IF,MEM_imm_update_unchanged_EX_jump,
       EX_data_rec_update_unchanged_IF,EX_jump_sel_addr_update_unchanged_IF,
       EX_SHIFT_update_unchanged_IF,EX_ALU_update_unchanged_IF,
       EX_compute_enable_update_unchanged_IF,EX_ALU_input_update_unchanged_IF,
@@ -696,7 +895,7 @@ Proof
      (`enable_stg 4 (agp32 fext fbits t)`
         by fs [enable_stg_def,agp32_IF_PC_write_enable_and_MEM_flag] >>
       fs [is_sch_def,is_sch_fetch_def,is_sch_memory_def] >>
-      Cases_on `isMemOp_isa_op (I' (4,t)) a` >> fs [] >>
+      Cases_on `isMemOp_hw_op (agp32 fext fbits t)` >> fs [] >>
       METIS_TAC []) >>
     Cases_on `isJump_isa_op (I' (1,t)) a \/ isJump_isa_op (I' (2,t)) a \/
     I' (1,t) = NONE \/ THE (I' (1,t)) = 0` >-
@@ -704,13 +903,13 @@ Proof
     fs [] >>
     `enable_stg 4 (agp32 fext fbits t)`
       by fs [enable_stg_def,agp32_IF_PC_write_enable_and_MEM_flag] >>
-    Cases_on `isMemOp_isa_op (I' (4,t)) a` >-
+    Cases_on `isMemOp_hw_op (agp32 fext fbits t)` >-
      (fs [is_sch_def,is_sch_memory_def] >> METIS_TAC []) >>
     `I' (4,SUC t) = I' (3,t)` by fs [is_sch_def,is_sch_memory_def] >> fs [] >>
     `(THE (I' (1,t)) > THE (I' (3,t))) /\ (THE (I' (1,t)) < THE (I' (3,t)) + 3)`
       by METIS_TAC [IF_instr_index_with_EX_instr] >> fs [is_sch_def,is_sch_fetch_def]) >>
   Cases_on `enable_stg 4 (agp32 fext fbits t)` >-
-   (Cases_on `isMemOp_isa_op (I' (4,t)) a` >-
+   (Cases_on `isMemOp_hw_op (agp32 fext fbits t)` >-
      (fs [is_sch_def,is_sch_memory_def] >> METIS_TAC []) >>
     `I' (4,SUC t) = I' (3,t)` by METIS_TAC [is_sch_def,is_sch_memory_def] >> fs [] >>
     `I' (1,SUC t) = I' (1,t)` by fs [is_sch_def,is_sch_disable_def] >> fs [] >>
@@ -763,12 +962,12 @@ Proof
     `I' (2,SUC t) = I' (1,t)` by fs [is_sch_def,is_sch_decode_def] >>
     `enable_stg 4 (agp32 fext fbits t)`
       by fs [enable_stg_def,agp32_ID_ID_write_enable_MEM_state_flag] >>
-    Cases_on `isMemOp_isa_op (I' (4,t)) a` >-
+    Cases_on `isMemOp_hw_op (agp32 fext fbits t)` >-
      (fs [is_sch_def,is_sch_memory_def] >> METIS_TAC []) >>
     `I' (4,SUC t) = I' (3,t)` by fs [is_sch_def,is_sch_memory_def] >> fs [] >>
     METIS_TAC [IF_instr_index_with_EX_instr]) >>
   Cases_on `enable_stg 4 (agp32 fext fbits t)` >-
-   (Cases_on `isMemOp_isa_op (I' (4,t)) a` >-
+   (Cases_on `isMemOp_hw_op (agp32 fext fbits t)` >-
      (fs [is_sch_def,is_sch_memory_def] >> METIS_TAC []) >>
     `I' (2,SUC t) = I' (2,t) /\ I' (4,SUC t) = I' (3,t)`
       by fs [is_sch_def,is_sch_memory_def,is_sch_disable_def] >> fs [] >>
@@ -811,7 +1010,7 @@ Theorem EX_instr_index_with_MEM_instr:
     is_sch I (agp32 fext fbits) a ==>
     I (3,t) <> NONE ==>
     I (4,t) <> NONE ==>
-    (THE (I (3,t)) >= THE (I (4,t))) /\ (THE (I (3,t)) < THE (I (4,t)) + 2)
+    (THE (I (3,t)) > THE (I (4,t))) /\ (THE (I (3,t)) < THE (I (4,t)) + 2)
 Proof
   rpt gen_tac >> rpt disch_tac >>
   Induct_on `t` >-
@@ -823,17 +1022,16 @@ Proof
     `I' (3,SUC t) = I' (2,t)` by fs [is_sch_def,is_sch_execute_def] >> fs [] >>
     `enable_stg 4 (agp32 fext fbits t)`
       by fs [enable_stg_def,agp32_ID_EX_write_enable_MEM_state_flag] >>
-    Cases_on `isMemOp_isa_op (I' (4,t)) a` >-
+    Cases_on `isMemOp_hw_op (agp32 fext fbits t)` >-
      (fs [is_sch_def,is_sch_memory_def] >> METIS_TAC []) >>
     `I' (4,SUC t) = I' (3,t)` by fs [is_sch_def,is_sch_memory_def] >> fs [] >>
-    `(THE (I' (2,t)) > THE (I' (3,t))) /\ (THE (I' (2,t)) < THE (I' (3,t)) + 2)`
-      by METIS_TAC [ID_instr_index_with_EX_instr] >> fs []) >>
+    METIS_TAC [ID_instr_index_with_EX_instr]) >>
   Cases_on `enable_stg 4 (agp32 fext fbits t)` >>
   fs [is_sch_def,is_sch_disable_def] >-
-   (Cases_on `isMemOp_isa_op (I' (4,t)) a` >-
+   (Cases_on `isMemOp_hw_op (agp32 fext fbits t)` >-
      (fs [is_sch_memory_def] >> METIS_TAC []) >>
-    `I' (4,SUC t) = I' (3,t)` by fs [is_sch_memory_def] >> fs []) >>
-  `I' (3,SUC t) = I' (3,t) /\ I' (4,SUC t) = I' (4,t)` by fs [] >> fs []
+    fs [enable_stg_def] >> METIS_TAC [agp32_ID_EX_write_disable_MEM_state_enable_MEM_stg_op]) >>
+  METIS_TAC []
 QED
 
 (** instr index relation between EX and WB stages **)
@@ -842,7 +1040,7 @@ Theorem EX_instr_index_with_WB_instr:
     is_sch I (agp32 fext fbits) a ==>
     I (3,t) <> NONE ==>
     I (5,t) <> NONE ==>
-    (THE (I (3,t)) >= THE (I (5,t))) /\ (THE (I (3,t)) < THE (I (5,t)) + 3)
+    (THE (I (3,t)) > THE (I (5,t))) /\ (THE (I (3,t)) < THE (I (5,t)) + 3)
 Proof
   rpt gen_tac >> rpt disch_tac >>
   Induct_on `t` >-
@@ -860,7 +1058,7 @@ Proof
   Cases_on `enable_stg 5 (agp32 fext fbits t)` >-
   (`I' (3,SUC t) = I' (3,t) /\ I' (5,SUC t) = I' (4,t)`
      by fs [is_sch_def,is_sch_writeback_def,is_sch_disable_def] >> fs [] >>
-   `(THE (I' (3,t)) >= THE (I' (4,t))) /\ (THE (I' (3,t)) < THE (I' (4,t)) + 2)`
+   `(THE (I' (3,t)) > THE (I' (4,t))) /\ (THE (I' (3,t)) < THE (I' (4,t)) + 2)`
      by METIS_TAC [EX_instr_index_with_MEM_instr] >> fs []) >>
   `I' (3,SUC t) = I' (3,t) /\ I' (5,SUC t) = I' (5,t)`
     by fs [is_sch_def,is_sch_disable_def] >> fs []
@@ -872,14 +1070,14 @@ Theorem MEM_instr_index_with_WB_instr:
     is_sch I (agp32 fext fbits) a ==>
     I (4,t) <> NONE ==>
     I (5,t) <> NONE ==>
-    (THE (I (4,t)) >= THE (I (5,t))) /\ (THE (I (4,t)) < THE (I (5,t)) + 2)
+    (THE (I (4,t)) > THE (I (5,t))) /\ (THE (I (4,t)) < THE (I (5,t)) + 2)
 Proof
   rpt gen_tac >> rpt disch_tac >>
   Induct_on `t` >-
    fs [is_sch_def,is_sch_init_def] >>
   rpt disch_tac >>
   Cases_on `enable_stg 4 (agp32 fext fbits t)` >-
-   (Cases_on `isMemOp_isa_op (I' (4,t)) a` >-
+   (Cases_on `isMemOp_hw_op (agp32 fext fbits t)` >-
      (fs [is_sch_def,is_sch_memory_def] >> METIS_TAC []) >>
     `I' (4,SUC t) = I' (3,t)` by fs [is_sch_def,is_sch_memory_def] >> fs [] >>
     `enable_stg 4 (agp32 fext fbits t)`
@@ -912,7 +1110,7 @@ Proof
       `I' (1,SUC t) = SOME (THE (I' (3,t)) + 1) /\ I' (5,SUC t) = I' (4,t)`
         by fs [is_sch_def,is_sch_fetch_def,is_sch_writeback_def] >> fs [] >>
       `I' (3,t) <> NONE` by METIS_TAC [isJump_isa_op_not_none] >>
-      `(THE (I' (3,t)) >= THE (I' (4,t))) /\ (THE (I' (3,t)) < THE (I' (4,t)) + 2)`
+      `(THE (I' (3,t)) > THE (I' (4,t))) /\ (THE (I' (3,t)) < THE (I' (4,t)) + 2)`
         by METIS_TAC [EX_instr_index_with_MEM_instr] >> fs []) >>
     Cases_on `isJump_isa_op (I' (1,t)) a \/ isJump_isa_op (I' (2,t)) a \/
     I' (1,t) = NONE \/ THE (I' (1,t)) = 0` >-
@@ -958,6 +1156,32 @@ Proof
     by METIS_TAC [ID_instr_index_with_EX_instr] >> fs []
 QED
 
+(** I (3,t) = I (4,t) + 1 **)
+Theorem EX_instr_index_with_MEM_instr_plus_1:
+  !I t fext fbits a.
+    is_sch I (agp32 fext fbits) a ==>
+    I (3,t) <> NONE ==>
+    I (4,t) <> NONE ==>
+    THE (I (3,t)) = THE (I (4,t)) + 1
+Proof
+  rw [] >>
+  `(THE (I' (3,t)) > THE (I' (4,t))) /\ (THE (I' (3,t)) < THE (I' (4,t)) + 2)`
+    by METIS_TAC [EX_instr_index_with_MEM_instr] >> fs []
+QED
+
+(** I (4,t) = I (5,t) + 1 **)
+Theorem MEM_instr_index_with_WB_instr_plus_1:
+  !I t fext fbits a.
+    is_sch I (agp32 fext fbits) a ==>
+    I (4,t) <> NONE ==>
+    I (5,t) <> NONE ==>
+    THE (I (4,t)) = THE (I (5,t)) + 1
+Proof
+  rw [] >>
+  `(THE (I' (4,t)) > THE (I' (5,t))) /\ (THE (I' (4,t)) < THE (I' (5,t)) + 2)`
+    by METIS_TAC [MEM_instr_index_with_WB_instr] >> fs []
+QED
+
 (** I (3,SUC t) = I (3,t) + 1 **)
 Theorem EX_instr_index_t_SUC_t_enable:
   !I t fext fbits a.
@@ -973,30 +1197,33 @@ Proof
   METIS_TAC [ID_instr_index_with_EX_instr_plus_1]
 QED
 
-(** I (3,t) = I (4,t) \/ (I (4,t) + 1) **)
-Theorem EX_instr_index_with_MEM_instr_plus_1:
+(** I (4,SUC t) = I (4,t) + 1 **)
+Theorem MEM_instr_index_t_SUC_t_enable:
   !I t fext fbits a.
     is_sch I (agp32 fext fbits) a ==>
-    I (3,t) <> NONE ==>
+    enable_stg 4 (agp32 fext fbits t) ==>
     I (4,t) <> NONE ==>
-    (THE (I (3,t)) = THE (I (4,t)) + 1) \/ (THE (I (3,t)) = THE (I (4,t)))
+    I (4,SUC t) <> NONE ==>
+    THE (I (4,SUC t)) = THE (I (4,t)) + 1
 Proof
-  rw [] >>
-  `(THE (I' (3,t)) >= THE (I' (4,t))) /\ (THE (I' (3,t)) < THE (I' (4,t)) + 2)`
-    by METIS_TAC [EX_instr_index_with_MEM_instr] >> fs []
+  rw [] >> Cases_on `isMemOp_hw_op (agp32 fext fbits t)` >-
+   (fs [is_sch_def,is_sch_memory_def] >> METIS_TAC []) >>
+  `I' (4,SUC t) = I' (3,t)` by fs [is_sch_def,is_sch_memory_def] >> fs [] >>
+  METIS_TAC [EX_instr_index_with_MEM_instr_plus_1]
 QED
 
-(** I (4,t) = I (5,t) \/ (I (5,t) + 1) **)
-Theorem MEM_instr_index_with_WB_instr_plus_1:
+(** I (5,SUC t) = I (5,t) + 1 **)
+Theorem WB_instr_index_t_SUC_t_enable:
   !I t fext fbits a.
     is_sch I (agp32 fext fbits) a ==>
-    I (4,t) <> NONE ==>
+    enable_stg 5 (agp32 fext fbits t) ==>
     I (5,t) <> NONE ==>
-    (THE (I (4,t)) = THE (I (5,t)) + 1) \/ (THE (I (4,t)) = THE (I (5,t)))
+    I (5,SUC t) <> NONE ==>
+    THE (I (5,SUC t)) = THE (I (5,t)) + 1
 Proof
   rw [] >>
-  `(THE (I' (4,t)) >= THE (I' (5,t))) /\ (THE (I' (4,t)) < THE (I' (5,t)) + 2)`
-    by METIS_TAC [MEM_instr_index_with_WB_instr] >> fs []
+  `I' (5,SUC t) = I' (4,t)` by fs [is_sch_def,is_sch_writeback_def] >> fs [] >>
+  METIS_TAC [MEM_instr_index_with_WB_instr_plus_1]
 QED
 
 
@@ -1077,7 +1304,7 @@ Proof
     `I' (2,SUC t) = I' (1,t)` by fs [is_sch_def,is_sch_decode_def] >>
     `enable_stg 4 (agp32 fext fbits t)`
       by fs [enable_stg_def,agp32_ID_ID_write_enable_MEM_state_flag] >>
-    Cases_on `isMemOp_isa_op (I' (4,t)) a` >-
+    Cases_on `isMemOp_hw_op (agp32 fext fbits t)` >-
      (fs [is_sch_def,is_sch_memory_def] >> METIS_TAC []) >>
     `I' (4,SUC t) = I' (3,t)` by fs [is_sch_def,is_sch_memory_def] >> fs [] >>
     `enable_stg 3 (agp32 fext fbits t)`
@@ -1085,7 +1312,7 @@ Proof
     `I' (3,SUC t) = I' (2,t)` by METIS_TAC [is_sch_def,is_sch_execute_def] >>
     fs [] >> METIS_TAC [IF_EX_instr_NOT_NONE_ID_NOT_NONE]) >>
   Cases_on `enable_stg 4 (agp32 fext fbits t)` >-
-   (Cases_on `isMemOp_isa_op (I' (4,t)) a` >-
+   (Cases_on `isMemOp_hw_op (agp32 fext fbits t)` >-
      (fs [is_sch_def,is_sch_memory_def] >> METIS_TAC []) >>
     `I' (2,SUC t) = I' (2,t) /\ I' (4,SUC t) = I' (3,t)`
       by fs [is_sch_def,is_sch_memory_def,is_sch_disable_def] >> fs [] >>
@@ -1110,27 +1337,6 @@ Proof
     by METIS_TAC [ID_instr_index_with_MEM_instr_EX_NONE] >> fs []
 QED
 
-(*
-Theorem test1[local]:
-  !I t fext fbits a.
-    is_sch I (agp32 fext fbits) a ==>
-    I (4,t) <> NONE ==>
-    (agp32 fext fbits t).MEM.MEM_opc = opc (FUNPOW Next (THE (I (4,t)) - 1) a)
-Proof
-  rw [is_sch_def] >>
-  Induct_on `t` >-
-   fs [is_sch_init_def] >>
-  rw [] >> Cases_on `enable_stg 4 (agp32 fext fbits t)` >-
-   (fs [is_sch_memory_def] >>
-    Cases_on `isMemOp_isa_op (I' (4,t)) a` >- METIS_TAC [] >>
-    `I' (4,SUC t) = I' (3,t)` by fs [] >>
-    `(agp32 fext fbits (SUC t)).MEM.MEM_opc = (agp32 fext fbits t).EX.EX_opc` by cheat >>
-    fs [] >> cheat)
-   fs [is_sch_disable_def] >>
-  `I' (4,SUC t) = I' (4,t)` by fs [] >>
-  `(agp32 fext fbits (SUC t)).MEM.MEM_opc = (agp32 fext fbits t).MEM.MEM_opc` by cheat >> fs []
-QED
-*)
 
 (** instr index relation between ID and MEM stages when EX is NONE **)
 Theorem EX_instr_index_with_WB_instr_MEM_NONE:
@@ -1139,7 +1345,7 @@ Theorem EX_instr_index_with_WB_instr_MEM_NONE:
     I (3,t) <> NONE ==>
     I (4,t) = NONE ==>
     I (5,t) <> NONE ==>
-    (THE (I (3,t)) >= THE (I (5,t))) /\ (THE (I (3,t)) < THE (I (5,t)) + 2)
+    (THE (I (3,t)) > THE (I (5,t))) /\ (THE (I (3,t)) < THE (I (5,t)) + 2)
 Proof
   rpt gen_tac >> rpt disch_tac >>
   Induct_on `t` >-
@@ -1154,10 +1360,8 @@ Proof
     `I' (5,SUC t) = I' (4,t)` by fs [is_sch_def,is_sch_writeback_def] >> fs [] >>
     `enable_stg 4 (agp32 fext fbits t)`
       by fs [enable_stg_def,agp32_ID_EX_write_enable_MEM_state_flag] >>
-    Cases_on `isMemOp_isa_op (I' (4,t)) a` >-
-     (`(agp32 fext fbits t).MEM.MEM_opc = opc (FUNPOW Next (THE (I' (4,t)) - 1) a)` by cheat >>
-      `(agp32 fext fbits t).ID.ID_EX_write_enable` by fs [enable_stg_def] >>
-      fs [isMemOp_isa_op_def,isMEM_stg_op_isa_def] >>
+    Cases_on `isMemOp_hw_op (agp32 fext fbits t)` >-
+     (fs [enable_stg_def] >>
       METIS_TAC [agp32_ID_EX_write_enable_no_MEM_stg_op]) >>
     `I' (4,SUC t) = I' (3,t)` by METIS_TAC [is_sch_def,is_sch_memory_def] >> fs [] >>
     `(THE (I' (2,t)) > THE (I' (4,t))) /\ (THE (I' (2,t)) < THE (I' (4,t)) + 2)`
@@ -1167,7 +1371,7 @@ Proof
       by fs [is_sch_def,is_sch_disable_def] >> fs [] >>
     `enable_stg 4 (agp32 fext fbits t)`
       by fs [enable_stg_def,agp32_MEM_state_flag_eq_WB_state_flag] >>
-    Cases_on `isMemOp_isa_op (I' (4,t)) a` >-
+    Cases_on `isMemOp_hw_op (agp32 fext fbits t)` >-
      (`I' (5,SUC t) = I' (4,t)` by fs [is_sch_def,is_sch_writeback_def] >> fs [] >>
       METIS_TAC [EX_instr_index_with_MEM_instr]) >>
     fs [is_sch_def,is_sch_memory_def] >> METIS_TAC []) >>
@@ -1176,17 +1380,17 @@ Proof
   fs [is_sch_def,is_sch_disable_def] >> METIS_TAC []
 QED
 
-(** I (3,t) = I (5,t) \/ (I (5,t) + 1) **)
+(** I (3,t) = I (5,t) + 1 when I (4,t) is NONE **)
 Theorem EX_instr_index_with_WB_instr_plus_1_MEM_NONE:
   !I t fext fbits a.
     is_sch I (agp32 fext fbits) a ==>
     I (3,t) <> NONE ==>
     I (4,t) = NONE ==>
     I (5,t) <> NONE ==>
-    (THE (I (3,t)) = THE (I (5,t)) + 1) \/ (THE (I (3,t)) = THE (I (5,t)))
+    THE (I (3,t)) = THE (I (5,t)) + 1
 Proof
   rw [] >>
-  `(THE (I' (3,t)) >= THE (I' (5,t))) /\ (THE (I' (3,t)) < THE (I' (5,t)) + 2)`
+  `(THE (I' (3,t)) > THE (I' (5,t))) /\ (THE (I' (3,t)) < THE (I' (5,t)) + 2)`
     by METIS_TAC [EX_instr_index_with_WB_instr_MEM_NONE] >> fs []
 QED
 
@@ -1209,7 +1413,7 @@ Proof
      (`enable_stg 4 (agp32 fext fbits t)`
         by fs [enable_stg_def,agp32_IF_PC_write_enable_and_MEM_flag] >>
       fs [is_sch_def,is_sch_fetch_def,is_sch_memory_def] >>
-      Cases_on `isMemOp_isa_op (I' (4,t)) a` >> fs [] >>
+      Cases_on `isMemOp_hw_op (agp32 fext fbits t)` >> fs [] >>
       METIS_TAC []) >>
     Cases_on `isJump_isa_op (I' (1,t)) a \/ isJump_isa_op (I' (2,t)) a \/
     I' (1,t) = NONE \/ THE (I' (1,t)) = 0` >-
@@ -1219,7 +1423,7 @@ Proof
       by fs [enable_stg_def,agp32_IF_PC_write_enable_and_ID_ID_write_enable] >>
     `I' (2,SUC t) = I' (1,t)` by METIS_TAC [is_sch_def,is_sch_decode_def] >> fs []) >>
   Cases_on `enable_stg 4 (agp32 fext fbits t)` >-
-   (Cases_on `isMemOp_isa_op (I' (4,t)) a` >-
+   (Cases_on `isMemOp_hw_op (agp32 fext fbits t)` >-
      (fs [is_sch_def,is_sch_memory_def] >> METIS_TAC []) >>
     `I' (4,SUC t) = I' (3,t)` by fs [is_sch_def,is_sch_memory_def] >>
     `~enable_stg 3 (agp32 fext fbits t)`
@@ -1254,7 +1458,7 @@ Proof
     `I' (5,SUC t) = I' (4,t)` by fs [is_sch_def,is_sch_writeback_def] >> fs [] >>
     `enable_stg 4 (agp32 fext fbits t)`
       by fs [enable_stg_def,agp32_ID_ID_write_enable_MEM_state_flag] >>
-    Cases_on `isMemOp_isa_op (I' (4,t)) a` >-
+    Cases_on `isMemOp_hw_op (agp32 fext fbits t)` >-
      (`enable_stg 3 (agp32 fext fbits t)`
         by fs [enable_stg_def, agp32_ID_ID_write_enable_eq_ID_EX_write_enable] >>
       `I' (3,SUC t) = I' (2,t)` by METIS_TAC [is_sch_def,is_sch_execute_def] >> fs [] >>
@@ -1292,6 +1496,68 @@ Proof
   rw [] >>
   `(THE (I' (2,t)) > THE (I' (5,t))) /\ (THE (I' (2,t)) < THE (I' (5,t)) + 2)`
     by METIS_TAC [ID_instr_index_with_WB_instr_EX_MEM_NONE] >> fs []
+QED
+
+(** instr index relation between IF and WB stages when ID, EX and MEM are NONE **)
+Theorem IF_instr_index_with_WB_instr_ID_EX_MEM_NONE:
+  !I t fext fbits a.
+    is_sch I (agp32 fext fbits) a ==>
+    I (1,t) <> NONE ==>
+    I (2,t) = NONE ==>
+    I (3,t) = NONE ==>
+    I (4,t) = NONE ==>
+    I (5,t) <> NONE ==>
+    (THE (I (1,t)) > THE (I (5,t))) /\ (THE (I (1,t)) < THE (I (5,t)) + 2)
+Proof
+  rpt gen_tac >> rpt disch_tac >>
+  Induct_on `t` >-
+   fs [is_sch_def,is_sch_init_def] >>
+  rpt disch_tac >>
+  Cases_on `enable_stg 1 (agp32 fext fbits t)` >-
+   (Cases_on `isJump_isa_op (I' (3,t)) a` >-
+     (`I' (1,SUC t) = SOME (THE (I' (3,t)) + 1)` by fs [is_sch_def,is_sch_fetch_def] >>
+      `I' (3,t) <> NONE` by METIS_TAC [isJump_isa_op_not_none] >>
+      `enable_stg 4 (agp32 fext fbits t)`
+        by fs [enable_stg_def,agp32_IF_PC_write_enable_and_MEM_flag] >>
+      `enable_stg 3 (agp32 fext fbits t)`
+        by fs [enable_stg_def,agp32_IF_PC_write_enable_and_ID_EX_write_enable] >>
+      Cases_on `isMemOp_hw_op (agp32 fext fbits t)` >-
+       (fs [enable_stg_def] >>
+        METIS_TAC [MEM_stg_op_agp32_ID_EX_write_disable]) >>
+      `I' (4,SUC t) = I' (3,t)` by METIS_TAC [is_sch_def,is_sch_memory_def] >> fs []) >>
+    Cases_on `isJump_isa_op (I' (1,t)) a \/ isJump_isa_op (I' (2,t)) a \/
+    I' (1,t) = NONE \/ THE (I' (1,t)) = 0` >-
+     (fs [is_sch_def,is_sch_fetch_def,is_sch_execute_def] >> METIS_TAC []) >>
+    fs [] >>
+    `enable_stg 2 (agp32 fext fbits t)`
+      by fs [enable_stg_def,agp32_IF_PC_write_enable_and_ID_ID_write_enable] >>
+    `I' (2,SUC t) = I' (1,t)` by METIS_TAC [is_sch_def,is_sch_decode_def] >> fs []) >>
+  `~enable_stg 2 (agp32 fext fbits t) /\ ~enable_stg 3 (agp32 fext fbits t)`
+    by METIS_TAC [enable_stg_def,agp32_IF_PC_write_enable_and_ID_EX_write_enable,
+                  agp32_IF_PC_write_enable_and_ID_ID_write_enable] >>
+  Cases_on `enable_stg 5 (agp32 fext fbits t)` >-
+   (`I' (5,SUC t) = I' (4,t)` by fs [is_sch_def,is_sch_writeback_def] >>
+    `I' (1,SUC t) = I' (1,t) /\ I' (2,SUC t) = I' (2,t) /\ I' (3,SUC t) = I' (3,t)`
+      by METIS_TAC [is_sch_def,is_sch_disable_def] >> fs [] >>
+    METIS_TAC [IF_instr_index_with_MEM_instr_ID_EX_NONE]) >>
+  `~enable_stg 4 (agp32 fext fbits t)` by fs [enable_stg_def,agp32_MEM_state_flag_eq_WB_state_flag] >>
+  fs [is_sch_def,is_sch_disable_def] >> METIS_TAC []
+QED
+
+(** I (5,t) = I (1,t) + 1 when I (2,t), I (3,t) and I (4,t) are NONE **)
+Theorem ID_EX_MEM_NONE_IF_instr_index_with_WB_instr_plus_1:
+  !I t fext fbits a.
+    is_sch I (agp32 fext fbits) a ==>
+    I (1,t) <> NONE ==>
+    I (2,t) = NONE ==>
+    I (3,t) = NONE ==>
+    I (4,t) = NONE ==>
+    I (5,t) <> NONE ==>
+    THE (I (1,t)) = THE (I (5,t)) + 1
+Proof
+  rw [] >>
+  `(THE (I' (1,t)) > THE (I' (5,t))) /\ (THE (I' (1,t)) < THE (I' (5,t)) + 2)`
+    by METIS_TAC [IF_instr_index_with_WB_instr_ID_EX_MEM_NONE] >> fs []
 QED
 
 val _ = export_theory ();
