proof/agp32_ID_CorrectScript.sml
@@ -96,8 +96,8 @@ Proof
   Q.ABBREV_TAC `s = agp32 fext fbits t` >>
   Q.ABBREV_TAC `s' = procs [agp32_next_state; WB_pipeline; MEM_pipeline; EX_pipeline;
                             REG_write; ID_pipeline; IF_PC_update; Acc_compute] (fext t) s s` >>
-  Q.ABBREV_TAC `s'' = procs [ForwardA; ForwardB; ForwardW; IF_instr_update; ID_opc_func_update;
-                             ID_imm_update] (fext (SUC t)) s' s'` >>                          
+  Q.ABBREV_TAC `s'' = procs [ForwardA; ForwardB; ForwardW; IF_instr_update;
+                             WB_update; ID_opc_func_update; ID_imm_update] (fext (SUC t)) s' s'` >>
   `?s0. (agp32 fext fbits (SUC t)).ID.ID_addrA = (ID_data_update (fext (SUC t)) s0 s'').ID.ID_addrA /\
   (agp32 fext fbits (SUC t)).ID.ID_addrB = (ID_data_update (fext (SUC t)) s0 s'').ID.ID_addrB /\
   (agp32 fext fbits (SUC t)).ID.ID_addrW = (ID_data_update (fext (SUC t)) s0 s'').ID.ID_addrW`
@@ -126,8 +126,8 @@ Proof
   Q.ABBREV_TAC `s = agp32 fext fbits t` >>
   Q.ABBREV_TAC `s' = procs [agp32_next_state; WB_pipeline; MEM_pipeline; EX_pipeline;
                             REG_write; ID_pipeline; IF_PC_update; Acc_compute] (fext t) s s` >>
-  Q.ABBREV_TAC `s'' = procs [ForwardA; ForwardB; ForwardW; IF_instr_update; ID_opc_func_update;
-                             ID_imm_update] (fext (SUC t)) s' s'` >>                          
+  Q.ABBREV_TAC `s'' = procs [ForwardA; ForwardB; ForwardW; IF_instr_update;
+                             WB_update; ID_opc_func_update; ID_imm_update] (fext (SUC t)) s' s'` >>
   `((agp32 fext fbits (SUC t)).ID.ID_addrA_disable <=>
     (ID_data_update (fext (SUC t)) s' s'').ID.ID_addrA_disable) /\
   ((agp32 fext fbits (SUC t)).ID.ID_addrB_disable <=>
@@ -159,8 +159,8 @@ Proof
   Q.ABBREV_TAC `s = agp32 fext fbits t` >>
   Q.ABBREV_TAC `s' = procs [agp32_next_state; WB_pipeline; MEM_pipeline; EX_pipeline;
                             REG_write; ID_pipeline; IF_PC_update; Acc_compute] (fext t) s s` >>
-  Q.ABBREV_TAC `s'' = procs [ForwardA; ForwardB; ForwardW; IF_instr_update; ID_opc_func_update;
-                             ID_imm_update] (fext (SUC t)) s' s'` >>                          
+  Q.ABBREV_TAC `s'' = procs [ForwardA; ForwardB; ForwardW; IF_instr_update;
+                             WB_update; ID_opc_func_update; ID_imm_update] (fext (SUC t)) s' s'` >>
   `(agp32 fext fbits (SUC t)).ID.ID_immA = (ID_data_update (fext (SUC t)) s' s'').ID.ID_immA /\
   (agp32 fext fbits (SUC t)).ID.ID_immB = (ID_data_update (fext (SUC t)) s' s'').ID.ID_immB /\
   (agp32 fext fbits (SUC t)).ID.ID_immW = (ID_data_update (fext (SUC t)) s' s'').ID.ID_immW`
@@ -186,8 +186,8 @@ Proof
   Q.ABBREV_TAC `s = agp32 fext fbits t` >>
   Q.ABBREV_TAC `s' = procs [agp32_next_state; WB_pipeline; MEM_pipeline; EX_pipeline;
                             REG_write; ID_pipeline; IF_PC_update; Acc_compute] (fext t) s s` >>
-  Q.ABBREV_TAC `s'' = procs [ForwardA; ForwardB; ForwardW; IF_instr_update; ID_opc_func_update]
-                            (fext (SUC t)) s' s'` >>
+  Q.ABBREV_TAC `s'' = procs [ForwardA; ForwardB; ForwardW; IF_instr_update;
+                             WB_update; ID_opc_func_update] (fext (SUC t)) s' s'` >>
   `(agp32 fext fbits (SUC t)).ID.ID_imm = (ID_imm_update (fext (SUC t)) s' s'').ID.ID_imm`
     by fs [Abbr `s`,Abbr `s'`,Abbr `s''`,agp32_ID_imm_updated_by_ID_imm_update] >>
   `s''.ID.ID_instr = (agp32 fext fbits (SUC t)).ID.ID_instr`
@@ -211,7 +211,8 @@ Proof
   Q.ABBREV_TAC `s = agp32 fext fbits t` >>
   Q.ABBREV_TAC `s' = procs [agp32_next_state; WB_pipeline; MEM_pipeline; EX_pipeline;
                             REG_write; ID_pipeline; IF_PC_update; Acc_compute] (fext t) s s` >>
-  Q.ABBREV_TAC `s'' = procs [ForwardA; ForwardB; ForwardW; IF_instr_update] (fext (SUC t)) s' s'` >>
+  Q.ABBREV_TAC `s'' = procs [ForwardA; ForwardB; ForwardW;
+                             IF_instr_update; WB_update] (fext (SUC t)) s' s'` >>
   `?s0.(agp32 fext fbits (SUC t)).ID.ID_opc = (ID_opc_func_update (fext (SUC t)) s0 s'').ID.ID_opc`
     by fs [Abbr `s`,Abbr `s'`,Abbr `s''`,agp32_ID_opc_func_updated_by_ID_opc_func_update] >>
   `s''.ID.ID_instr = (agp32 fext fbits (SUC t)).ID.ID_instr`
@@ -284,7 +285,8 @@ Proof
   Q.ABBREV_TAC `s = agp32 fext fbits t` >>
   Q.ABBREV_TAC `s' = procs [agp32_next_state; WB_pipeline; MEM_pipeline; EX_pipeline;
                             REG_write; ID_pipeline; IF_PC_update; Acc_compute] (fext t) s s` >>
-  Q.ABBREV_TAC `s'' = procs [ForwardA; ForwardB; ForwardW; IF_instr_update] (fext (SUC t)) s' s'` >>
+  Q.ABBREV_TAC `s'' = procs [ForwardA; ForwardB; ForwardW;
+                             IF_instr_update; WB_update] (fext (SUC t)) s' s'` >>
   `?s0.
     (agp32 fext fbits (SUC t)).ID.ID_opc = (ID_opc_func_update (fext (SUC t)) s0 s'').ID.ID_opc /\
   (agp32 fext fbits (SUC t)).ID.ID_func = (ID_opc_func_update (fext (SUC t)) s0 s'').ID.ID_func`
@@ -392,8 +394,8 @@ Proof
   fs [enable_stg_def] >> Q.ABBREV_TAC `s = agp32 fext fbits t` >>
   Q.ABBREV_TAC `s' = procs [agp32_next_state; WB_pipeline; MEM_pipeline; EX_pipeline;
                             REG_write; ID_pipeline; IF_PC_update; Acc_compute] (fext t) s s` >>
-  Q.ABBREV_TAC `s'' = procs [ForwardA; ForwardB; ForwardW; IF_instr_update; ID_opc_func_update;
-                             ID_imm_update] (fext (SUC t)) s' s'` >>
+  Q.ABBREV_TAC `s'' = procs [ForwardA; ForwardB; ForwardW; IF_instr_update;
+                             WB_update; ID_opc_func_update; ID_imm_update] (fext (SUC t)) s' s'` >>
   `((agp32 fext fbits (SUC t)).ID.ID_ForwardA = (ID_data_update (fext (SUC t)) s' s'').ID.ID_ForwardA) /\
   ((agp32 fext fbits (SUC t)).ID.ID_ForwardB = (ID_data_update (fext (SUC t)) s' s'').ID.ID_ForwardB) /\
   ((agp32 fext fbits (SUC t)).ID.ID_ForwardW = (ID_data_update (fext (SUC t)) s' s'').ID.ID_ForwardW)`
@@ -421,6 +423,51 @@ Proof
 QED
 
 
+
+(** lemmas about ID_Forward flags and reg_adr_update_isa **)
+Theorem agp32_ID_ForwardA_flag_reg_adr_update_isa:
+  !I fext fbits t a.
+    enable_stg 2 (agp32 fext fbits t) ==>
+    reg_adr_update_isa (I (5,SUC t)) a (agp32 fext fbits (SUC t)).ID.ID_addrA =
+    (agp32 fext fbits (SUC t)).ID.ID_ForwardA
+Proof
+  rw [agp32_Rel_ag32_ID_Forward_flags_correct,enable_stg_def] >>
+  fs [agp32_ID_ID_write_enable_WB_state_flag] >>
+  rw [reg_adr_update_isa_def] >>
+  Cases_on `I' (5,SUC t) = NONE` >-
+   (rw [] >> cheat) >>
+  rw [] >> cheat
+QED
+
+Theorem agp32_ID_ForwardB_flag_reg_adr_update_isa:
+  !I fext fbits t a.
+    enable_stg 2 (agp32 fext fbits t) ==>
+    reg_adr_update_isa (I (5,SUC t)) a (agp32 fext fbits (SUC t)).ID.ID_addrB =
+    (agp32 fext fbits (SUC t)).ID.ID_ForwardB
+Proof
+  rw [agp32_Rel_ag32_ID_Forward_flags_correct,enable_stg_def] >>
+  fs [agp32_ID_ID_write_enable_WB_state_flag] >>
+  rw [reg_adr_update_isa_def] >>
+  Cases_on `I' (5,SUC t) = NONE` >-
+   (rw [] >> cheat) >>
+  rw [] >> cheat
+QED
+
+Theorem agp32_ID_ForwardW_flag_reg_adr_update_isa:
+  !I fext fbits t a.
+    enable_stg 2 (agp32 fext fbits t) ==>
+    reg_adr_update_isa (I (5,SUC t)) a (agp32 fext fbits (SUC t)).ID.ID_addrW =
+    (agp32 fext fbits (SUC t)).ID.ID_ForwardW
+Proof
+  rw [agp32_Rel_ag32_ID_Forward_flags_correct,enable_stg_def] >>
+  fs [agp32_ID_ID_write_enable_WB_state_flag] >>
+  rw [reg_adr_update_isa_def] >>
+  Cases_on `I' (5,SUC t) = NONE` >-
+   (rw [] >> cheat) >>
+  rw [] >> cheat
+QED
+
+
 (** ID_read_dataA: when instrs in EX, MEM and WB do not change registers **)
 Theorem agp32_Rel_ag32_ID_read_dataA_no_write_before:
   !fext fbits a t I.
@@ -439,8 +486,8 @@ Proof
   Q.ABBREV_TAC `s = agp32 fext fbits t` >>
   Q.ABBREV_TAC `s' = procs [agp32_next_state; WB_pipeline; MEM_pipeline; EX_pipeline;
                             REG_write; ID_pipeline; IF_PC_update; Acc_compute] (fext t) s s` >>
-  Q.ABBREV_TAC `s'' = procs [ForwardA; ForwardB; ForwardW; IF_instr_update; ID_opc_func_update;
-                             ID_imm_update] (fext (SUC t)) s' s'` >>                          
+  Q.ABBREV_TAC `s'' = procs [ForwardA; ForwardB; ForwardW; IF_instr_update;
+                             WB_update; ID_opc_func_update; ID_imm_update] (fext (SUC t)) s' s'` >>
   `(agp32 fext fbits (SUC t)).ID.ID_read_dataA =
   (ID_data_update (fext (SUC t)) s' s'').ID.ID_read_dataA`
     by fs [Abbr `s`,Abbr `s'`,Abbr `s''`,agp32_ID_read_data_updated_by_ID_data_update] >>
@@ -454,8 +501,11 @@ Proof
   Cases_on `I' (5,SUC t) = NONE` >>
   Cases_on `I' (4,SUC t) = NONE` >>
   Cases_on `I' (3,SUC t) = NONE` >-
+   (** 16 cases **)
+   (** all NONE **)
    (`(agp32 fext fbits (SUC t)).R = (FUNPOW Next (THE (I' (2,SUC t)) − 1) a).R`
-      by cheat >> fs []) >-      
+      by cheat >> fs []) >-
+   (** I (3,SUC t) is not NONE **)
    (`(agp32 fext fbits (SUC t)).R = (FUNPOW Next (THE (I' (3,SUC t)) − 1) a).R`
       by cheat >> fs [] >>
     `(agp32 fext fbits (SUC t)).ID.ID_addrA = (22 >< 17) i`
@@ -463,6 +513,7 @@ Proof
     `THE (I' (2,SUC t)) = THE (I' (3,SUC t)) + 1`
       by METIS_TAC [ID_instr_index_with_EX_instr_plus_1] >> fs [] >>
     METIS_TAC [reg_adr_update_isa_not_change_data]) >-
+   (** I (4,SUC t) is not NONE **)
    (`(agp32 fext fbits (SUC t)).R = (FUNPOW Next (THE (I' (4,SUC t)) − 1) a).R`
       by cheat >> fs [] >>
     `(agp32 fext fbits (SUC t)).ID.ID_addrA = (22 >< 17) i`
@@ -473,6 +524,7 @@ Proof
       by METIS_TAC [reg_adr_update_isa_not_change_data] >> fs [] >>
     `THE (I' (2,SUC t)) = THE (I' (4,SUC t)) + 1`
       by METIS_TAC [EX_NONE_ID_instr_index_with_MEM_instr_plus_1] >> fs []) >-
+   (** I (3,SUC t) and I (4,SUC t) are not NONE **)
    (`(agp32 fext fbits (SUC t)).R = (FUNPOW Next (THE (I' (4,SUC t)) − 1) a).R`
       by cheat >> fs [] >>
     `(agp32 fext fbits (SUC t)).ID.ID_addrA = (22 >< 17) i`
@@ -483,10 +535,11 @@ Proof
       by METIS_TAC [reg_adr_update_isa_not_change_data] >> fs [] >>
     `THE (I' (2,SUC t)) = THE (I' (3,SUC t)) + 1`
       by METIS_TAC [ID_instr_index_with_EX_instr_plus_1] >> fs [] >>
-    `(THE (I' (3,SUC t)) = THE (I' (4,SUC t))) \/ (THE (I' (3,SUC t)) = THE (I' (4,SUC t)) + 1)`
+    `THE (I' (3,SUC t)) = THE (I' (4,SUC t)) + 1`
       by METIS_TAC [EX_instr_index_with_MEM_instr_plus_1] >> fs [] >>
     `THE (I' (4,SUC t)) = THE (I' (3,SUC t)) - 1` by fs [] >> fs [] >>
     METIS_TAC [reg_adr_update_isa_not_change_data]) >-
+   (** I (5,SUC t) is not NONE **)
    (`(agp32 fext fbits (SUC t)).R = (FUNPOW Next (THE (I' (5,SUC t)) − 1) a).R`
       by cheat >> fs [] >>
     `(agp32 fext fbits (SUC t)).ID.ID_addrA = (22 >< 17) i`
@@ -497,6 +550,7 @@ Proof
       by METIS_TAC [reg_adr_update_isa_not_change_data] >> fs [] >>
     `THE (I' (2,SUC t)) = THE (I' (5,SUC t)) + 1`
       by METIS_TAC [EX_MEM_NONE_ID_instr_index_with_WB_instr_plus_1] >> fs []) >-
+   (** I (3,SUC t) and I (5,SUC t) are not NONE **)
    (`(agp32 fext fbits (SUC t)).R = (FUNPOW Next (THE (I' (5,SUC t)) − 1) a).R`
       by cheat >> fs [] >>
     `(agp32 fext fbits (SUC t)).ID.ID_addrA = (22 >< 17) i`
@@ -505,12 +559,13 @@ Proof
     `(FUNPOW Next (THE (I' (5,SUC t)) − 1) a).R ((22 >< 17) i) =
     (FUNPOW Next (THE (I' (5,SUC t))) a).R ((22 >< 17) i)`
       by METIS_TAC [reg_adr_update_isa_not_change_data] >> fs [] >>
-    `THE (I' (3,SUC t)) = THE (I' (5,SUC t)) + 1 \/ THE (I' (3,SUC t)) = THE (I' (5,SUC t))`
+    `THE (I' (3,SUC t)) = THE (I' (5,SUC t)) + 1`
       by METIS_TAC [EX_instr_index_with_WB_instr_plus_1_MEM_NONE] >>
     `THE (I' (2,SUC t)) = THE (I' (3,SUC t)) + 1`
       by METIS_TAC [ID_instr_index_with_EX_instr_plus_1] >> fs [] >>
     `THE (I' (5,SUC t)) = THE (I' (3,SUC t)) - 1` by fs [] >> fs [] >>
     METIS_TAC [reg_adr_update_isa_not_change_data]) >-
+   (** I (4,SUC t) and I (5,SUC t) are not NONE **)
    (`(agp32 fext fbits (SUC t)).R = (FUNPOW Next (THE (I' (5,SUC t)) − 1) a).R`
       by cheat >> fs [] >>
     `(agp32 fext fbits (SUC t)).ID.ID_addrA = (22 >< 17) i`
@@ -519,12 +574,13 @@ Proof
     `(FUNPOW Next (THE (I' (5,SUC t)) − 1) a).R ((22 >< 17) i) =
     (FUNPOW Next (THE (I' (5,SUC t))) a).R ((22 >< 17) i)`
       by METIS_TAC [reg_adr_update_isa_not_change_data] >> fs [] >>
-    `THE (I' (4,SUC t)) = THE (I' (5,SUC t)) + 1 \/ THE (I' (4,SUC t)) = THE (I' (5,SUC t))`
+    `THE (I' (4,SUC t)) = THE (I' (5,SUC t)) + 1`
       by METIS_TAC [MEM_instr_index_with_WB_instr_plus_1] >>
     `THE (I' (2,SUC t)) = THE (I' (4,SUC t)) + 1`
       by METIS_TAC [EX_NONE_ID_instr_index_with_MEM_instr_plus_1] >> fs [] >>
-    `THE (I' (5,SUC t)) = THE (I' (4,SUC t)) - 1` by fs [] >> fs [] >-
+    `THE (I' (5,SUC t)) = THE (I' (4,SUC t)) - 1` by fs [] >> fs [] >>
     METIS_TAC [reg_adr_update_isa_not_change_data]) >-
+   (** I (3,SUC t), I (4,SUC t) and I (5,SUC t) are not NONE **)
    (`(agp32 fext fbits (SUC t)).R = (FUNPOW Next (THE (I' (5,SUC t)) − 1) a).R`
       by cheat >> fs [] >>
     `(agp32 fext fbits (SUC t)).ID.ID_addrA = (22 >< 17) i`
@@ -533,28 +589,1040 @@ Proof
     `(FUNPOW Next (THE (I' (5,SUC t)) − 1) a).R ((22 >< 17) i) =
     (FUNPOW Next (THE (I' (5,SUC t))) a).R ((22 >< 17) i)`
       by METIS_TAC [reg_adr_update_isa_not_change_data] >> fs [] >>
-    `THE (I' (4,SUC t)) = THE (I' (5,SUC t)) + 1 \/ THE (I' (4,SUC t)) = THE (I' (5,SUC t))`
-      by METIS_TAC [MEM_instr_index_with_WB_instr_plus_1] >-
-     (`THE (I' (5,SUC t)) = THE (I' (4,SUC t)) - 1` by fs [] >> fs [] >>
-      `(FUNPOW Next (THE (I' (4,SUC t)) − 1) a).R ((22 >< 17) i) =
-      (FUNPOW Next (THE (I' (4,SUC t))) a).R ((22 >< 17) i)`
-        by METIS_TAC [reg_adr_update_isa_not_change_data] >> fs [] >>
-      `THE (I' (3,SUC t)) = THE (I' (4,SUC t)) \/ THE (I' (3,SUC t)) = THE (I' (4,SUC t)) + 1`
-        by METIS_TAC [EX_instr_index_with_MEM_instr_plus_1] >>
-      `THE (I' (2,SUC t)) = THE (I' (3,SUC t)) + 1`
-        by METIS_TAC [ID_instr_index_with_EX_instr_plus_1] >> fs [] >>
-      `THE (I' (4,SUC t)) = THE (I' (3,SUC t)) - 1` by FULL_SIMP_TAC std_ss [] >>
-      METIS_TAC [reg_adr_update_isa_not_change_data]) >>
-    `THE (I' (3,SUC t)) = THE (I' (4,SUC t)) \/ THE (I' (3,SUC t)) = THE (I' (4,SUC t)) + 1`
+    `THE (I' (4,SUC t)) = THE (I' (5,SUC t)) + 1`
+      by METIS_TAC [MEM_instr_index_with_WB_instr_plus_1] >>
+    `THE (I' (5,SUC t)) = THE (I' (4,SUC t)) - 1` by fs [] >> fs [] >>
+    `(FUNPOW Next (THE (I' (4,SUC t)) − 1) a).R ((22 >< 17) i) =
+    (FUNPOW Next (THE (I' (4,SUC t))) a).R ((22 >< 17) i)`
+      by METIS_TAC [reg_adr_update_isa_not_change_data] >> fs [] >>
+    `THE (I' (3,SUC t)) = THE (I' (4,SUC t)) + 1`
       by METIS_TAC [EX_instr_index_with_MEM_instr_plus_1] >>
     `THE (I' (2,SUC t)) = THE (I' (3,SUC t)) + 1`
       by METIS_TAC [ID_instr_index_with_EX_instr_plus_1] >> fs [] >>
     `THE (I' (4,SUC t)) = THE (I' (3,SUC t)) - 1` by FULL_SIMP_TAC std_ss [] >>
     METIS_TAC [reg_adr_update_isa_not_change_data]) >-
+   (** I (5,t) is not NONE **)
    (`s.WB.WB_state_flag` by fs [Abbr `s`,enable_stg_def,agp32_ID_ID_write_enable_WB_state_flag] >>
     `reg_data_vaild 5 s` by fs [Abbr `s`,reg_data_vaild_def] >>
     `(agp32 fext fbits (SUC t)).R = (FUNPOW Next (THE (I' (5,t))) a).R` by cheat >> fs [] >>
-    cheat) >>
+    subgoal `I' (2,SUC t) = I' (1,t)` >-
+     (fs [is_sch_def,is_sch_decode_def,Abbr `s`] >>
+      Cases_on `isJump_isa_op (I' (2,t)) a \/ isJump_isa_op (I' (3,t)) a` >>
+      METIS_TAC []) >> fs [] >>
+    subgoal `I' (5,SUC t) = I' (4,t)` >-
+     (fs [is_sch_def,is_sch_writeback_def,is_sch_disable_def,Abbr `s`] >>
+      Cases_on `enable_stg 5 (agp32 fext fbits t)` >>
+      METIS_TAC []) >> fs [] >>
+    subgoal `I' (4,SUC t) = I' (3,t)` >-
+     (fs [is_sch_def,is_sch_memory_def,Abbr `s`] >>
+      `enable_stg 4 (agp32 fext fbits t)`
+        by fs [enable_stg_def,agp32_ID_ID_write_enable_MEM_state_flag] >>
+      Cases_on `isMemOp_hw_op (agp32 fext fbits t)` >>
+      fs [enable_stg_def] >>
+      METIS_TAC [MEM_stg_op_agp32_ID_EX_write_disable,
+                 agp32_ID_ID_write_enable_eq_ID_EX_write_enable]) >> fs [] >>
+    subgoal `I' (3,SUC t) = I' (2,t)` >-
+     (fs [is_sch_def,is_sch_execute_def,Abbr `s`] >>
+      `enable_stg 3 (agp32 fext fbits t)`
+        by fs [enable_stg_def,agp32_ID_ID_write_enable_eq_ID_EX_write_enable] >>
+      Cases_on `isJump_isa_op (I' (3,t)) a` >>
+      METIS_TAC [isJump_isa_op_not_none]) >> fs [] >>
+    `THE (I' (1,t)) = THE (I' (5,t)) + 1`
+      by METIS_TAC [ID_EX_MEM_NONE_IF_instr_index_with_WB_instr_plus_1] >> fs []) >-
+   (** I (3,SUC t) and I (5,t) are not NONE **)
+   (`s.WB.WB_state_flag` by fs [Abbr `s`,enable_stg_def,agp32_ID_ID_write_enable_WB_state_flag] >>
+    `reg_data_vaild 5 s` by fs [Abbr `s`,reg_data_vaild_def] >>
+    `(agp32 fext fbits (SUC t)).R = (FUNPOW Next (THE (I' (5,t))) a).R` by cheat >> fs [] >>
+    `(agp32 fext fbits (SUC t)).ID.ID_addrA = (22 >< 17) i`
+      by (fs [Abbr `i`,Abbr `s`,is_sch_def] >>
+          METIS_TAC [agp32_Rel_ag32_ID_addr_correct,addrA_def]) >> fs [] >>
+    subgoal `I' (2,SUC t) = I' (1,t)` >-
+     (fs [is_sch_def,is_sch_decode_def,Abbr `s`] >>
+      Cases_on `isJump_isa_op (I' (2,t)) a \/ isJump_isa_op (I' (3,t)) a` >>
+      METIS_TAC []) >> fs [] >>
+    subgoal `I' (5,SUC t) = I' (4,t)` >-
+     (fs [is_sch_def,is_sch_writeback_def,is_sch_disable_def,Abbr `s`] >>
+      Cases_on `enable_stg 5 (agp32 fext fbits t)` >>
+      METIS_TAC []) >> fs [] >>
+    subgoal `I' (4,SUC t) = I' (3,t)` >-
+     (fs [is_sch_def,is_sch_memory_def,Abbr `s`] >>
+      `enable_stg 4 (agp32 fext fbits t)`
+        by fs [enable_stg_def,agp32_ID_ID_write_enable_MEM_state_flag] >>
+      Cases_on `isMemOp_hw_op (agp32 fext fbits t)` >>
+      fs [enable_stg_def] >>
+      METIS_TAC [MEM_stg_op_agp32_ID_EX_write_disable,
+                 agp32_ID_ID_write_enable_eq_ID_EX_write_enable]) >> fs [] >>
+    subgoal `I' (3,SUC t) = I' (2,t)` >-
+     (fs [is_sch_def,is_sch_execute_def,Abbr `s`] >>
+      `enable_stg 3 (agp32 fext fbits t)`
+        by fs [enable_stg_def,agp32_ID_ID_write_enable_eq_ID_EX_write_enable] >>
+      Cases_on `isJump_isa_op (I' (3,t)) a` >>
+      METIS_TAC [isJump_isa_op_not_none]) >> fs [] >>
+    `THE (I' (2,t)) = THE (I' (5,t)) + 1`
+      by METIS_TAC [EX_MEM_NONE_ID_instr_index_with_WB_instr_plus_1] >>
+    `THE (I' (5,t)) = THE (I' (2,t)) - 1` by fs [] >>
+    `THE (I' (1,t)) = THE (I' (2,t)) + 1`
+      by METIS_TAC [IF_instr_index_with_ID_instr_plus_1] >> fs [] >>
+    METIS_TAC [reg_adr_update_isa_not_change_data]) >-
+   (** I (4,SUC t) and I (5,t) are not NONE **)
+   (`s.WB.WB_state_flag` by fs [Abbr `s`,enable_stg_def,agp32_ID_ID_write_enable_WB_state_flag] >>
+    `reg_data_vaild 5 s` by fs [Abbr `s`,reg_data_vaild_def] >>
+    `(agp32 fext fbits (SUC t)).R = (FUNPOW Next (THE (I' (5,t))) a).R` by cheat >> fs [] >>
+    `(agp32 fext fbits (SUC t)).ID.ID_addrA = (22 >< 17) i`
+      by (fs [Abbr `i`,Abbr `s`,is_sch_def] >>
+          METIS_TAC [agp32_Rel_ag32_ID_addr_correct,addrA_def]) >> fs [] >>
+    subgoal `THE (I' (4,SUC t)) = THE (I' (5,t)) + 1` >-
+     (`I' (5,SUC t) = I' (4,t)`
+        by (fs [is_sch_def,is_sch_writeback_def,is_sch_disable_def,Abbr `s`] >>
+            Cases_on `enable_stg 5 (agp32 fext fbits t)` >>
+            METIS_TAC []) >>
+      `I' (4,SUC t) = I' (3,t)`
+          by (fs [is_sch_def,is_sch_memory_def,Abbr `s`] >>
+              `enable_stg 4 (agp32 fext fbits t)`
+                by fs [enable_stg_def,agp32_ID_ID_write_enable_MEM_state_flag] >>
+              Cases_on `isMemOp_hw_op (agp32 fext fbits t)` >>
+              fs [enable_stg_def] >>
+              METIS_TAC [MEM_stg_op_agp32_ID_EX_write_disable,
+                         agp32_ID_ID_write_enable_eq_ID_EX_write_enable]) >> fs [] >>
+      METIS_TAC [EX_instr_index_with_WB_instr_plus_1_MEM_NONE]) >>
+    `THE (I' (5,t)) = THE (I' (4,SUC t)) - 1` by fs [] >> fs [] >>
+    `(FUNPOW Next (THE (I' (4,SUC t)) − 1) a).R ((22 >< 17) i) =
+    (FUNPOW Next (THE (I' (4,SUC t))) a).R ((22 >< 17) i)`
+      by METIS_TAC [reg_adr_update_isa_not_change_data] >> fs [] >>
+    `THE (I' (2,SUC t)) = THE (I' (4,SUC t)) + 1`
+      by METIS_TAC [EX_NONE_ID_instr_index_with_MEM_instr_plus_1] >> fs []) >-
+   (** I (3,SUC t), I (4,SUC t) and I (5,t) are not NONE **)
+   (`s.WB.WB_state_flag` by fs [Abbr `s`,enable_stg_def,agp32_ID_ID_write_enable_WB_state_flag] >>
+    `reg_data_vaild 5 s` by fs [Abbr `s`,reg_data_vaild_def] >>
+    `(agp32 fext fbits (SUC t)).R = (FUNPOW Next (THE (I' (5,t))) a).R` by cheat >> fs [] >>
+    `(agp32 fext fbits (SUC t)).ID.ID_addrA = (22 >< 17) i`
+      by (fs [Abbr `i`,Abbr `s`,is_sch_def] >>
+          METIS_TAC [agp32_Rel_ag32_ID_addr_correct,addrA_def]) >> fs [] >>
+    subgoal `THE (I' (4,SUC t)) = THE (I' (5,t)) + 1` >-
+     (`I' (5,SUC t) = I' (4,t)`
+        by (fs [is_sch_def,is_sch_writeback_def,is_sch_disable_def,Abbr `s`] >>
+            Cases_on `enable_stg 5 (agp32 fext fbits t)` >>
+            METIS_TAC []) >>
+      `I' (4,SUC t) = I' (3,t)`
+          by (fs [is_sch_def,is_sch_memory_def,Abbr `s`] >>
+              `enable_stg 4 (agp32 fext fbits t)`
+                by fs [enable_stg_def,agp32_ID_ID_write_enable_MEM_state_flag] >>
+              Cases_on `isMemOp_hw_op (agp32 fext fbits t)` >>
+              fs [enable_stg_def] >>
+              METIS_TAC [MEM_stg_op_agp32_ID_EX_write_disable,
+                         agp32_ID_ID_write_enable_eq_ID_EX_write_enable]) >> fs [] >>
+      METIS_TAC [EX_instr_index_with_WB_instr_plus_1_MEM_NONE]) >>
+    `THE (I' (5,t)) = THE (I' (4,SUC t)) - 1` by fs [] >> fs [] >>
+    `(FUNPOW Next (THE (I' (4,SUC t)) − 1) a).R ((22 >< 17) i) =
+    (FUNPOW Next (THE (I' (4,SUC t))) a).R ((22 >< 17) i)`
+      by METIS_TAC [reg_adr_update_isa_not_change_data] >> fs [] >>
+    `THE (I' (3,SUC t)) = THE (I' (4,SUC t)) + 1`
+      by METIS_TAC [EX_instr_index_with_MEM_instr_plus_1] >>
+    `THE (I' (2,SUC t)) = THE (I' (3,SUC t)) + 1`
+      by METIS_TAC [ID_instr_index_with_EX_instr_plus_1] >> fs [] >>
+    `THE (I' (4,SUC t)) = THE (I' (3,SUC t)) - 1` by FULL_SIMP_TAC std_ss [] >>
+    METIS_TAC [reg_adr_update_isa_not_change_data]) >-
+   (** I (5,SUC t) and I (5,t) are not NONE **)
+   (`s.WB.WB_state_flag` by fs [Abbr `s`,enable_stg_def,agp32_ID_ID_write_enable_WB_state_flag] >>
+    `reg_data_vaild 5 s` by fs [Abbr `s`,reg_data_vaild_def] >>
+    `(agp32 fext fbits (SUC t)).R = (FUNPOW Next (THE (I' (5,t))) a).R` by cheat >> fs [] >>
+    `(agp32 fext fbits (SUC t)).ID.ID_addrA = (22 >< 17) i`
+      by (fs [Abbr `i`,Abbr `s`,is_sch_def] >>
+          METIS_TAC [agp32_Rel_ag32_ID_addr_correct,addrA_def]) >> fs [] >>
+    `enable_stg 5 (agp32 fext fbits t)`
+      by fs [enable_stg_def,agp32_ID_ID_write_enable_WB_state_flag] >>
+    `THE (I' (5,SUC t)) = THE (I' (5,t)) + 1` by METIS_TAC [WB_instr_index_t_SUC_t_enable] >>
+    `THE (I' (5,t)) = THE (I' (5,SUC t)) - 1` by fs [] >> fs [] >>
+    `(FUNPOW Next (THE (I' (5,SUC t)) − 1) a).R ((22 >< 17) i) =
+    (FUNPOW Next (THE (I' (5,SUC t))) a).R ((22 >< 17) i)`
+      by METIS_TAC [reg_adr_update_isa_not_change_data] >> fs [] >>
+    `THE (I' (2,SUC t)) = THE (I' (5,SUC t)) + 1`
+      by METIS_TAC [EX_MEM_NONE_ID_instr_index_with_WB_instr_plus_1] >> fs []) >-
+   (** I (3,SUC t), I (5,SUC t) and I (5,t) are not NONE **)
+   (`s.WB.WB_state_flag` by fs [Abbr `s`,enable_stg_def,agp32_ID_ID_write_enable_WB_state_flag] >>
+    `reg_data_vaild 5 s` by fs [Abbr `s`,reg_data_vaild_def] >>
+    `(agp32 fext fbits (SUC t)).R = (FUNPOW Next (THE (I' (5,t))) a).R` by cheat >> fs [] >>
+    `(agp32 fext fbits (SUC t)).ID.ID_addrA = (22 >< 17) i`
+      by (fs [Abbr `i`,Abbr `s`,is_sch_def] >>
+          METIS_TAC [agp32_Rel_ag32_ID_addr_correct,addrA_def]) >> fs [] >>
+    `enable_stg 5 (agp32 fext fbits t)`
+      by fs [enable_stg_def,agp32_ID_ID_write_enable_WB_state_flag] >>
+    `THE (I' (5,SUC t)) = THE (I' (5,t)) + 1` by METIS_TAC [WB_instr_index_t_SUC_t_enable] >>
+    `THE (I' (5,t)) = THE (I' (5,SUC t)) - 1` by fs [] >> fs [] >>
+    `(FUNPOW Next (THE (I' (5,SUC t)) − 1) a).R ((22 >< 17) i) =
+    (FUNPOW Next (THE (I' (5,SUC t))) a).R ((22 >< 17) i)`
+      by METIS_TAC [reg_adr_update_isa_not_change_data] >> fs [] >>
+    `THE (I' (3,SUC t)) = THE (I' (5,SUC t)) + 1`
+      by METIS_TAC [EX_instr_index_with_WB_instr_plus_1_MEM_NONE] >>
+    `THE (I' (2,SUC t)) = THE (I' (3,SUC t)) + 1`
+      by METIS_TAC [ID_instr_index_with_EX_instr_plus_1] >> fs [] >>
+    `THE (I' (5,SUC t)) = THE (I' (3,SUC t)) - 1` by fs [] >>
+    METIS_TAC [reg_adr_update_isa_not_change_data]) >-
+   (** I (4,SUC t), I (5,SUC t) and I (5,t) are not NONE **)
+   (`s.WB.WB_state_flag` by fs [Abbr `s`,enable_stg_def,agp32_ID_ID_write_enable_WB_state_flag] >>
+    `reg_data_vaild 5 s` by fs [Abbr `s`,reg_data_vaild_def] >>
+    `(agp32 fext fbits (SUC t)).R = (FUNPOW Next (THE (I' (5,t))) a).R` by cheat >> fs [] >>
+    `(agp32 fext fbits (SUC t)).ID.ID_addrA = (22 >< 17) i`
+      by (fs [Abbr `i`,Abbr `s`,is_sch_def] >>
+          METIS_TAC [agp32_Rel_ag32_ID_addr_correct,addrA_def]) >> fs [] >>
+    `enable_stg 5 (agp32 fext fbits t)`
+      by fs [enable_stg_def,agp32_ID_ID_write_enable_WB_state_flag] >>
+    `THE (I' (5,SUC t)) = THE (I' (5,t)) + 1` by METIS_TAC [WB_instr_index_t_SUC_t_enable] >>
+    `THE (I' (5,t)) = THE (I' (5,SUC t)) - 1` by fs [] >> fs [] >>
+    `(FUNPOW Next (THE (I' (5,SUC t)) − 1) a).R ((22 >< 17) i) =
+    (FUNPOW Next (THE (I' (5,SUC t))) a).R ((22 >< 17) i)`
+      by METIS_TAC [reg_adr_update_isa_not_change_data] >> fs [] >>
+    `THE (I' (4,SUC t)) = THE (I' (5,SUC t)) + 1`
+      by METIS_TAC [MEM_instr_index_with_WB_instr_plus_1] >>
+    `THE (I' (2,SUC t)) = THE (I' (4,SUC t)) + 1`
+      by METIS_TAC [EX_NONE_ID_instr_index_with_MEM_instr_plus_1] >> fs [] >>
+    `THE (I' (5,SUC t)) = THE (I' (4,SUC t)) - 1` by fs [] >>
+    METIS_TAC [reg_adr_update_isa_not_change_data]) >>
+  (** all are not NONE **)
+  `s.WB.WB_state_flag` by fs [Abbr `s`,enable_stg_def,agp32_ID_ID_write_enable_WB_state_flag] >>
+  `reg_data_vaild 5 s` by fs [Abbr `s`,reg_data_vaild_def] >>
+  `(agp32 fext fbits (SUC t)).R = (FUNPOW Next (THE (I' (5,t))) a).R` by cheat >> fs [] >>
+  `(agp32 fext fbits (SUC t)).ID.ID_addrA = (22 >< 17) i`
+    by (fs [Abbr `i`,Abbr `s`,is_sch_def] >>
+        METIS_TAC [agp32_Rel_ag32_ID_addr_correct,addrA_def]) >> fs [] >>
+  `enable_stg 5 (agp32 fext fbits t)`
+    by fs [enable_stg_def,agp32_ID_ID_write_enable_WB_state_flag] >>
+  `THE (I' (5,SUC t)) = THE (I' (5,t)) + 1` by METIS_TAC [WB_instr_index_t_SUC_t_enable] >>
+  `THE (I' (5,t)) = THE (I' (5,SUC t)) - 1` by fs [] >> fs [] >>
+  `(FUNPOW Next (THE (I' (5,SUC t)) − 1) a).R ((22 >< 17) i) =
+  (FUNPOW Next (THE (I' (5,SUC t))) a).R ((22 >< 17) i)`
+    by METIS_TAC [reg_adr_update_isa_not_change_data] >> fs [] >>
+  qpat_x_assum `THE (I' (5,SUC t)) = _` (fn thm => all_tac)  >>
+  `THE (I' (4,SUC t)) = THE (I' (5,SUC t)) + 1`
+    by METIS_TAC [MEM_instr_index_with_WB_instr_plus_1] >>
+  `THE (I' (5,SUC t)) = THE (I' (4,SUC t)) - 1` by fs [] >> fs [] >>
+  `(FUNPOW Next (THE (I' (4,SUC t)) − 1) a).R ((22 >< 17) i) =
+  (FUNPOW Next (THE (I' (4,SUC t))) a).R ((22 >< 17) i)`
+    by METIS_TAC [reg_adr_update_isa_not_change_data] >> fs [] >>
+  `THE (I' (3,SUC t)) = THE (I' (4,SUC t)) + 1`
+    by METIS_TAC [EX_instr_index_with_MEM_instr_plus_1] >>
+  `THE (I' (2,SUC t)) = THE (I' (3,SUC t)) + 1`
+    by METIS_TAC [ID_instr_index_with_EX_instr_plus_1] >> fs [] >>
+  `THE (I' (4,SUC t)) = THE (I' (3,SUC t)) - 1` by FULL_SIMP_TAC std_ss [] >>
+  METIS_TAC [reg_adr_update_isa_not_change_data]
+QED
+
+
+(** ID_read_dataB: when instrs in EX, MEM and WB do not change registers **)
+Theorem agp32_Rel_ag32_ID_read_dataB_no_write_before:
+  !fext fbits a t I.
+    is_sch I (agp32 fext fbits) a ==>
+    Rel I (fext t) (agp32 fext fbits (t-1)) (agp32 fext fbits t) a t ==>
+    enable_stg 2 (agp32 fext fbits t) ==>
+    I (2,SUC t) <> NONE ==>
+    ~reg_adr_update_isa (I (3,SUC t)) a (agp32 fext fbits (SUC t)).ID.ID_addrB ==>
+    ~reg_adr_update_isa (I (4,SUC t)) a (agp32 fext fbits (SUC t)).ID.ID_addrB ==>
+    ~reg_adr_update_isa (I (5,SUC t)) a (agp32 fext fbits (SUC t)).ID.ID_addrB ==>
+    (agp32 fext fbits (SUC t)).ID.ID_read_dataB = reg_dataB (FUNPOW Next (THE (I (2,SUC t)) − 1) a)
+Proof
+  rw [reg_dataB_def,addrB_def] >>
+  `(agp32 fext fbits (SUC t)).ID.ID_instr = instr (FUNPOW Next (THE (I' (2,SUC t)) − 1) a)`
+    by fs [is_sch_def,agp32_Rel_ag32_ID_instr_correct] >>
+  Q.ABBREV_TAC `s = agp32 fext fbits t` >>
+  Q.ABBREV_TAC `s' = procs [agp32_next_state; WB_pipeline; MEM_pipeline; EX_pipeline;
+                            REG_write; ID_pipeline; IF_PC_update; Acc_compute] (fext t) s s` >>
+  Q.ABBREV_TAC `s'' = procs [ForwardA; ForwardB; ForwardW; IF_instr_update;
+                             WB_update; ID_opc_func_update; ID_imm_update] (fext (SUC t)) s' s'` >>
+  `(agp32 fext fbits (SUC t)).ID.ID_read_dataB =
+  (ID_data_update (fext (SUC t)) s' s'').ID.ID_read_dataB`
+    by fs [Abbr `s`,Abbr `s'`,Abbr `s''`,agp32_ID_read_data_updated_by_ID_data_update] >>
+  fs [ID_data_update_def] >>
+  `s''.ID.ID_instr = (agp32 fext fbits (SUC t)).ID.ID_instr`
+    by fs [Abbr `s`,Abbr `s'`,Abbr `s''`,agp32_same_ID_instr_after_ID_imm_update] >> fs [] >>
+  qpat_abbrev_tac `i = instr _` >>
+  `s''.R = (agp32 fext fbits (SUC t)).R`
+    by fs [Abbr `s`,Abbr `s'`,Abbr `s''`,agp32_same_R_after_ID_imm_update] >> fs [] >>
+  Cases_on `I' (5,t) = NONE` >>
+  Cases_on `I' (5,SUC t) = NONE` >>
+  Cases_on `I' (4,SUC t) = NONE` >>
+  Cases_on `I' (3,SUC t) = NONE` >-
+   (** all NONE **)
+   (`(agp32 fext fbits (SUC t)).R = (FUNPOW Next (THE (I' (2,SUC t)) − 1) a).R`
+      by cheat >> fs []) >-
+   (** I (3,SUC t) is not NONE **)
+   (`(agp32 fext fbits (SUC t)).R = (FUNPOW Next (THE (I' (3,SUC t)) − 1) a).R`
+      by cheat >> fs [] >>
+    `(agp32 fext fbits (SUC t)).ID.ID_addrB = (15 >< 10) i`
+      by (fs [Abbr `i`,Abbr `s`,is_sch_def] >> METIS_TAC [agp32_Rel_ag32_ID_addr_correct,addrB_def]) >>
+    `THE (I' (2,SUC t)) = THE (I' (3,SUC t)) + 1`
+      by METIS_TAC [ID_instr_index_with_EX_instr_plus_1] >> fs [] >>
+    METIS_TAC [reg_adr_update_isa_not_change_data]) >-
+   (** I (4,SUC t) is not NONE **)
+   (`(agp32 fext fbits (SUC t)).R = (FUNPOW Next (THE (I' (4,SUC t)) − 1) a).R`
+      by cheat >> fs [] >>
+    `(agp32 fext fbits (SUC t)).ID.ID_addrB = (15 >< 10) i`
+      by (fs [Abbr `i`,Abbr `s`,is_sch_def] >> METIS_TAC [agp32_Rel_ag32_ID_addr_correct,addrB_def]) >>
+    fs [] >>
+    `(FUNPOW Next (THE (I' (4,SUC t)) − 1) a).R ((15 >< 10) i) =
+    (FUNPOW Next (THE (I' (4,SUC t))) a).R ((15 >< 10) i)`
+      by METIS_TAC [reg_adr_update_isa_not_change_data] >> fs [] >>
+    `THE (I' (2,SUC t)) = THE (I' (4,SUC t)) + 1`
+      by METIS_TAC [EX_NONE_ID_instr_index_with_MEM_instr_plus_1] >> fs []) >-
+   (** I (3,SUC t) and I (4,SUC t) are not NONE **)
+   (`(agp32 fext fbits (SUC t)).R = (FUNPOW Next (THE (I' (4,SUC t)) − 1) a).R`
+      by cheat >> fs [] >>
+    `(agp32 fext fbits (SUC t)).ID.ID_addrB = (15 >< 10) i`
+      by (fs [Abbr `i`,Abbr `s`,is_sch_def] >> METIS_TAC [agp32_Rel_ag32_ID_addr_correct,addrB_def]) >>
+    fs [] >>
+    `(FUNPOW Next (THE (I' (4,SUC t)) − 1) a).R ((15 >< 10) i) =
+    (FUNPOW Next (THE (I' (4,SUC t))) a).R ((15 >< 10) i)`
+      by METIS_TAC [reg_adr_update_isa_not_change_data] >> fs [] >>
+    `THE (I' (2,SUC t)) = THE (I' (3,SUC t)) + 1`
+      by METIS_TAC [ID_instr_index_with_EX_instr_plus_1] >> fs [] >>
+    `THE (I' (3,SUC t)) = THE (I' (4,SUC t)) + 1`
+      by METIS_TAC [EX_instr_index_with_MEM_instr_plus_1] >> fs [] >>
+    `THE (I' (4,SUC t)) = THE (I' (3,SUC t)) - 1` by fs [] >> fs [] >>
+    METIS_TAC [reg_adr_update_isa_not_change_data]) >-
+   (** I (5,SUC t) is not NONE **)
+   (`(agp32 fext fbits (SUC t)).R = (FUNPOW Next (THE (I' (5,SUC t)) − 1) a).R`
+      by cheat >> fs [] >>
+    `(agp32 fext fbits (SUC t)).ID.ID_addrB = (15 >< 10) i`
+      by (fs [Abbr `i`,Abbr `s`,is_sch_def] >>
+          METIS_TAC [agp32_Rel_ag32_ID_addr_correct,addrB_def]) >> fs [] >>
+    `(FUNPOW Next (THE (I' (5,SUC t)) − 1) a).R ((15 >< 10) i) =
+    (FUNPOW Next (THE (I' (5,SUC t))) a).R ((15 >< 10) i)`
+      by METIS_TAC [reg_adr_update_isa_not_change_data] >> fs [] >>
+    `THE (I' (2,SUC t)) = THE (I' (5,SUC t)) + 1`
+      by METIS_TAC [EX_MEM_NONE_ID_instr_index_with_WB_instr_plus_1] >> fs []) >-
+   (** I (3,SUC t) and I (5,SUC t) are not NONE **)
+   (`(agp32 fext fbits (SUC t)).R = (FUNPOW Next (THE (I' (5,SUC t)) − 1) a).R`
+      by cheat >> fs [] >>
+    `(agp32 fext fbits (SUC t)).ID.ID_addrB = (15 >< 10) i`
+      by (fs [Abbr `i`,Abbr `s`,is_sch_def] >>
+          METIS_TAC [agp32_Rel_ag32_ID_addr_correct,addrB_def]) >> fs [] >>
+    `(FUNPOW Next (THE (I' (5,SUC t)) − 1) a).R ((15 >< 10) i) =
+    (FUNPOW Next (THE (I' (5,SUC t))) a).R ((15 >< 10) i)`
+      by METIS_TAC [reg_adr_update_isa_not_change_data] >> fs [] >>
+    `THE (I' (3,SUC t)) = THE (I' (5,SUC t)) + 1`
+      by METIS_TAC [EX_instr_index_with_WB_instr_plus_1_MEM_NONE] >>
+    `THE (I' (2,SUC t)) = THE (I' (3,SUC t)) + 1`
+      by METIS_TAC [ID_instr_index_with_EX_instr_plus_1] >> fs [] >>
+    `THE (I' (5,SUC t)) = THE (I' (3,SUC t)) - 1` by fs [] >> fs [] >>
+    METIS_TAC [reg_adr_update_isa_not_change_data]) >-
+   (** I (4,SUC t) and I (5,SUC t) are not NONE **)
+   (`(agp32 fext fbits (SUC t)).R = (FUNPOW Next (THE (I' (5,SUC t)) − 1) a).R`
+      by cheat >> fs [] >>
+    `(agp32 fext fbits (SUC t)).ID.ID_addrB = (15 >< 10) i`
+      by (fs [Abbr `i`,Abbr `s`,is_sch_def] >>
+          METIS_TAC [agp32_Rel_ag32_ID_addr_correct,addrB_def]) >> fs [] >>
+    `(FUNPOW Next (THE (I' (5,SUC t)) − 1) a).R ((15 >< 10) i) =
+    (FUNPOW Next (THE (I' (5,SUC t))) a).R ((15 >< 10) i)`
+      by METIS_TAC [reg_adr_update_isa_not_change_data] >> fs [] >>
+    `THE (I' (4,SUC t)) = THE (I' (5,SUC t)) + 1`
+      by METIS_TAC [MEM_instr_index_with_WB_instr_plus_1] >>
+    `THE (I' (2,SUC t)) = THE (I' (4,SUC t)) + 1`
+      by METIS_TAC [EX_NONE_ID_instr_index_with_MEM_instr_plus_1] >> fs [] >>
+    `THE (I' (5,SUC t)) = THE (I' (4,SUC t)) - 1` by fs [] >> fs [] >>
+    METIS_TAC [reg_adr_update_isa_not_change_data]) >-
+   (** I (3,SUC t), I (4,SUC t) and I (5,SUC t) are not NONE **)
+   (`(agp32 fext fbits (SUC t)).R = (FUNPOW Next (THE (I' (5,SUC t)) − 1) a).R`
+      by cheat >> fs [] >>
+    `(agp32 fext fbits (SUC t)).ID.ID_addrB = (15 >< 10) i`
+      by (fs [Abbr `i`,Abbr `s`,is_sch_def] >>
+          METIS_TAC [agp32_Rel_ag32_ID_addr_correct,addrB_def]) >> fs [] >>
+    `(FUNPOW Next (THE (I' (5,SUC t)) − 1) a).R ((15 >< 10) i) =
+    (FUNPOW Next (THE (I' (5,SUC t))) a).R ((15 >< 10) i)`
+      by METIS_TAC [reg_adr_update_isa_not_change_data] >> fs [] >>
+    `THE (I' (4,SUC t)) = THE (I' (5,SUC t)) + 1`
+      by METIS_TAC [MEM_instr_index_with_WB_instr_plus_1] >>
+    `THE (I' (5,SUC t)) = THE (I' (4,SUC t)) - 1` by fs [] >> fs [] >>
+    `(FUNPOW Next (THE (I' (4,SUC t)) − 1) a).R ((15 >< 10) i) =
+    (FUNPOW Next (THE (I' (4,SUC t))) a).R ((15 >< 10) i)`
+      by METIS_TAC [reg_adr_update_isa_not_change_data] >> fs [] >>
+    `THE (I' (3,SUC t)) = THE (I' (4,SUC t)) + 1`
+      by METIS_TAC [EX_instr_index_with_MEM_instr_plus_1] >>
+    `THE (I' (2,SUC t)) = THE (I' (3,SUC t)) + 1`
+      by METIS_TAC [ID_instr_index_with_EX_instr_plus_1] >> fs [] >>
+    `THE (I' (4,SUC t)) = THE (I' (3,SUC t)) - 1` by FULL_SIMP_TAC std_ss [] >>
+    METIS_TAC [reg_adr_update_isa_not_change_data]) >-
+   (** I (5,t) is not NONE **)
+   (`s.WB.WB_state_flag` by fs [Abbr `s`,enable_stg_def,agp32_ID_ID_write_enable_WB_state_flag] >>
+    `reg_data_vaild 5 s` by fs [Abbr `s`,reg_data_vaild_def] >>
+    `(agp32 fext fbits (SUC t)).R = (FUNPOW Next (THE (I' (5,t))) a).R` by cheat >> fs [] >>
+    subgoal `I' (2,SUC t) = I' (1,t)` >-
+     (fs [is_sch_def,is_sch_decode_def,Abbr `s`] >>
+      Cases_on `isJump_isa_op (I' (2,t)) a \/ isJump_isa_op (I' (3,t)) a` >>
+      METIS_TAC []) >> fs [] >>
+    subgoal `I' (5,SUC t) = I' (4,t)` >-
+     (fs [is_sch_def,is_sch_writeback_def,is_sch_disable_def,Abbr `s`] >>
+      Cases_on `enable_stg 5 (agp32 fext fbits t)` >>
+      METIS_TAC []) >> fs [] >>
+    subgoal `I' (4,SUC t) = I' (3,t)` >-
+     (fs [is_sch_def,is_sch_memory_def,Abbr `s`] >>
+      `enable_stg 4 (agp32 fext fbits t)`
+        by fs [enable_stg_def,agp32_ID_ID_write_enable_MEM_state_flag] >>
+      Cases_on `isMemOp_hw_op (agp32 fext fbits t)` >>
+      fs [enable_stg_def] >>
+      METIS_TAC [MEM_stg_op_agp32_ID_EX_write_disable,
+                 agp32_ID_ID_write_enable_eq_ID_EX_write_enable]) >> fs [] >>
+    subgoal `I' (3,SUC t) = I' (2,t)` >-
+     (fs [is_sch_def,is_sch_execute_def,Abbr `s`] >>
+      `enable_stg 3 (agp32 fext fbits t)`
+        by fs [enable_stg_def,agp32_ID_ID_write_enable_eq_ID_EX_write_enable] >>
+      Cases_on `isJump_isa_op (I' (3,t)) a` >>
+      METIS_TAC [isJump_isa_op_not_none]) >> fs [] >>
+    `THE (I' (1,t)) = THE (I' (5,t)) + 1`
+      by METIS_TAC [ID_EX_MEM_NONE_IF_instr_index_with_WB_instr_plus_1] >> fs []) >-
+   (** I (3,SUC t) and I (5,t) are not NONE **)
+   (`s.WB.WB_state_flag` by fs [Abbr `s`,enable_stg_def,agp32_ID_ID_write_enable_WB_state_flag] >>
+    `reg_data_vaild 5 s` by fs [Abbr `s`,reg_data_vaild_def] >>
+    `(agp32 fext fbits (SUC t)).R = (FUNPOW Next (THE (I' (5,t))) a).R` by cheat >> fs [] >>
+    `(agp32 fext fbits (SUC t)).ID.ID_addrB = (15 >< 10) i`
+      by (fs [Abbr `i`,Abbr `s`,is_sch_def] >>
+          METIS_TAC [agp32_Rel_ag32_ID_addr_correct,addrB_def]) >> fs [] >>
+    subgoal `I' (2,SUC t) = I' (1,t)` >-
+     (fs [is_sch_def,is_sch_decode_def,Abbr `s`] >>
+      Cases_on `isJump_isa_op (I' (2,t)) a \/ isJump_isa_op (I' (3,t)) a` >>
+      METIS_TAC []) >> fs [] >>
+    subgoal `I' (5,SUC t) = I' (4,t)` >-
+     (fs [is_sch_def,is_sch_writeback_def,is_sch_disable_def,Abbr `s`] >>
+      Cases_on `enable_stg 5 (agp32 fext fbits t)` >>
+      METIS_TAC []) >> fs [] >>
+    subgoal `I' (4,SUC t) = I' (3,t)` >-
+     (fs [is_sch_def,is_sch_memory_def,Abbr `s`] >>
+      `enable_stg 4 (agp32 fext fbits t)`
+        by fs [enable_stg_def,agp32_ID_ID_write_enable_MEM_state_flag] >>
+      Cases_on `isMemOp_hw_op (agp32 fext fbits t)` >>
+      fs [enable_stg_def] >>
+      METIS_TAC [MEM_stg_op_agp32_ID_EX_write_disable,
+                 agp32_ID_ID_write_enable_eq_ID_EX_write_enable]) >> fs [] >>
+    subgoal `I' (3,SUC t) = I' (2,t)` >-
+     (fs [is_sch_def,is_sch_execute_def,Abbr `s`] >>
+      `enable_stg 3 (agp32 fext fbits t)`
+        by fs [enable_stg_def,agp32_ID_ID_write_enable_eq_ID_EX_write_enable] >>
+      Cases_on `isJump_isa_op (I' (3,t)) a` >>
+      METIS_TAC [isJump_isa_op_not_none]) >> fs [] >>
+    `THE (I' (2,t)) = THE (I' (5,t)) + 1`
+      by METIS_TAC [EX_MEM_NONE_ID_instr_index_with_WB_instr_plus_1] >>
+    `THE (I' (5,t)) = THE (I' (2,t)) - 1` by fs [] >>
+    `THE (I' (1,t)) = THE (I' (2,t)) + 1`
+      by METIS_TAC [IF_instr_index_with_ID_instr_plus_1] >> fs [] >>
+    METIS_TAC [reg_adr_update_isa_not_change_data]) >-
+   (** I (4,SUC t) and I (5,t) are not NONE **)
+   (`s.WB.WB_state_flag` by fs [Abbr `s`,enable_stg_def,agp32_ID_ID_write_enable_WB_state_flag] >>
+    `reg_data_vaild 5 s` by fs [Abbr `s`,reg_data_vaild_def] >>
+    `(agp32 fext fbits (SUC t)).R = (FUNPOW Next (THE (I' (5,t))) a).R` by cheat >> fs [] >>
+    `(agp32 fext fbits (SUC t)).ID.ID_addrB = (15 >< 10) i`
+      by (fs [Abbr `i`,Abbr `s`,is_sch_def] >>
+          METIS_TAC [agp32_Rel_ag32_ID_addr_correct,addrB_def]) >> fs [] >>
+    subgoal `THE (I' (4,SUC t)) = THE (I' (5,t)) + 1` >-
+     (`I' (5,SUC t) = I' (4,t)`
+        by (fs [is_sch_def,is_sch_writeback_def,is_sch_disable_def,Abbr `s`] >>
+            Cases_on `enable_stg 5 (agp32 fext fbits t)` >>
+            METIS_TAC []) >>
+      `I' (4,SUC t) = I' (3,t)`
+          by (fs [is_sch_def,is_sch_memory_def,Abbr `s`] >>
+              `enable_stg 4 (agp32 fext fbits t)`
+                by fs [enable_stg_def,agp32_ID_ID_write_enable_MEM_state_flag] >>
+              Cases_on `isMemOp_hw_op (agp32 fext fbits t)` >>
+              fs [enable_stg_def] >>
+              METIS_TAC [MEM_stg_op_agp32_ID_EX_write_disable,
+                         agp32_ID_ID_write_enable_eq_ID_EX_write_enable]) >> fs [] >>
+      METIS_TAC [EX_instr_index_with_WB_instr_plus_1_MEM_NONE]) >>
+    `THE (I' (5,t)) = THE (I' (4,SUC t)) - 1` by fs [] >> fs [] >>
+    `(FUNPOW Next (THE (I' (4,SUC t)) − 1) a).R ((15 >< 10) i) =
+    (FUNPOW Next (THE (I' (4,SUC t))) a).R ((15 >< 10) i)`
+      by METIS_TAC [reg_adr_update_isa_not_change_data] >> fs [] >>
+    `THE (I' (2,SUC t)) = THE (I' (4,SUC t)) + 1`
+      by METIS_TAC [EX_NONE_ID_instr_index_with_MEM_instr_plus_1] >> fs []) >-
+   (** I (3,SUC t), I (4,SUC t) and I (5,t) are not NONE **)
+   (`s.WB.WB_state_flag` by fs [Abbr `s`,enable_stg_def,agp32_ID_ID_write_enable_WB_state_flag] >>
+    `reg_data_vaild 5 s` by fs [Abbr `s`,reg_data_vaild_def] >>
+    `(agp32 fext fbits (SUC t)).R = (FUNPOW Next (THE (I' (5,t))) a).R` by cheat >> fs [] >>
+    `(agp32 fext fbits (SUC t)).ID.ID_addrB = (15 >< 10) i`
+      by (fs [Abbr `i`,Abbr `s`,is_sch_def] >>
+          METIS_TAC [agp32_Rel_ag32_ID_addr_correct,addrB_def]) >> fs [] >>
+    subgoal `THE (I' (4,SUC t)) = THE (I' (5,t)) + 1` >-
+     (`I' (5,SUC t) = I' (4,t)`
+        by (fs [is_sch_def,is_sch_writeback_def,is_sch_disable_def,Abbr `s`] >>
+            Cases_on `enable_stg 5 (agp32 fext fbits t)` >>
+            METIS_TAC []) >>
+      `I' (4,SUC t) = I' (3,t)`
+          by (fs [is_sch_def,is_sch_memory_def,Abbr `s`] >>
+              `enable_stg 4 (agp32 fext fbits t)`
+                by fs [enable_stg_def,agp32_ID_ID_write_enable_MEM_state_flag] >>
+              Cases_on `isMemOp_hw_op (agp32 fext fbits t)` >>
+              fs [enable_stg_def] >>
+              METIS_TAC [MEM_stg_op_agp32_ID_EX_write_disable,
+                         agp32_ID_ID_write_enable_eq_ID_EX_write_enable]) >> fs [] >>
+      METIS_TAC [EX_instr_index_with_WB_instr_plus_1_MEM_NONE]) >>
+    `THE (I' (5,t)) = THE (I' (4,SUC t)) - 1` by fs [] >> fs [] >>
+    `(FUNPOW Next (THE (I' (4,SUC t)) − 1) a).R ((15 >< 10) i) =
+    (FUNPOW Next (THE (I' (4,SUC t))) a).R ((15 >< 10) i)`
+      by METIS_TAC [reg_adr_update_isa_not_change_data] >> fs [] >>
+    `THE (I' (3,SUC t)) = THE (I' (4,SUC t)) + 1`
+      by METIS_TAC [EX_instr_index_with_MEM_instr_plus_1] >>
+    `THE (I' (2,SUC t)) = THE (I' (3,SUC t)) + 1`
+      by METIS_TAC [ID_instr_index_with_EX_instr_plus_1] >> fs [] >>
+    `THE (I' (4,SUC t)) = THE (I' (3,SUC t)) - 1` by FULL_SIMP_TAC std_ss [] >>
+    METIS_TAC [reg_adr_update_isa_not_change_data]) >-
+   (** I (5,SUC t) and I (5,t) are not NONE **)
+   (`s.WB.WB_state_flag` by fs [Abbr `s`,enable_stg_def,agp32_ID_ID_write_enable_WB_state_flag] >>
+    `reg_data_vaild 5 s` by fs [Abbr `s`,reg_data_vaild_def] >>
+    `(agp32 fext fbits (SUC t)).R = (FUNPOW Next (THE (I' (5,t))) a).R` by cheat >> fs [] >>
+    `(agp32 fext fbits (SUC t)).ID.ID_addrB = (15 >< 10) i`
+      by (fs [Abbr `i`,Abbr `s`,is_sch_def] >>
+          METIS_TAC [agp32_Rel_ag32_ID_addr_correct,addrB_def]) >> fs [] >>
+    `enable_stg 5 (agp32 fext fbits t)`
+      by fs [enable_stg_def,agp32_ID_ID_write_enable_WB_state_flag] >>
+    `THE (I' (5,SUC t)) = THE (I' (5,t)) + 1` by METIS_TAC [WB_instr_index_t_SUC_t_enable] >>
+    `THE (I' (5,t)) = THE (I' (5,SUC t)) - 1` by fs [] >> fs [] >>
+    `(FUNPOW Next (THE (I' (5,SUC t)) − 1) a).R ((15 >< 10) i) =
+    (FUNPOW Next (THE (I' (5,SUC t))) a).R ((15 >< 10) i)`
+      by METIS_TAC [reg_adr_update_isa_not_change_data] >> fs [] >>
+    `THE (I' (2,SUC t)) = THE (I' (5,SUC t)) + 1`
+      by METIS_TAC [EX_MEM_NONE_ID_instr_index_with_WB_instr_plus_1] >> fs []) >-
+   (** I (3,SUC t), I (5,SUC t) and I (5,t) are not NONE **)
+   (`s.WB.WB_state_flag` by fs [Abbr `s`,enable_stg_def,agp32_ID_ID_write_enable_WB_state_flag] >>
+    `reg_data_vaild 5 s` by fs [Abbr `s`,reg_data_vaild_def] >>
+    `(agp32 fext fbits (SUC t)).R = (FUNPOW Next (THE (I' (5,t))) a).R` by cheat >> fs [] >>
+    `(agp32 fext fbits (SUC t)).ID.ID_addrB = (15 >< 10) i`
+      by (fs [Abbr `i`,Abbr `s`,is_sch_def] >>
+          METIS_TAC [agp32_Rel_ag32_ID_addr_correct,addrB_def]) >> fs [] >>
+    `enable_stg 5 (agp32 fext fbits t)`
+      by fs [enable_stg_def,agp32_ID_ID_write_enable_WB_state_flag] >>
+    `THE (I' (5,SUC t)) = THE (I' (5,t)) + 1` by METIS_TAC [WB_instr_index_t_SUC_t_enable] >>
+    `THE (I' (5,t)) = THE (I' (5,SUC t)) - 1` by fs [] >> fs [] >>
+    `(FUNPOW Next (THE (I' (5,SUC t)) − 1) a).R ((15 >< 10) i) =
+    (FUNPOW Next (THE (I' (5,SUC t))) a).R ((15 >< 10) i)`
+      by METIS_TAC [reg_adr_update_isa_not_change_data] >> fs [] >>
+    `THE (I' (3,SUC t)) = THE (I' (5,SUC t)) + 1`
+      by METIS_TAC [EX_instr_index_with_WB_instr_plus_1_MEM_NONE] >>
+    `THE (I' (2,SUC t)) = THE (I' (3,SUC t)) + 1`
+      by METIS_TAC [ID_instr_index_with_EX_instr_plus_1] >> fs [] >>
+    `THE (I' (5,SUC t)) = THE (I' (3,SUC t)) - 1` by fs [] >>
+    METIS_TAC [reg_adr_update_isa_not_change_data]) >-
+   (** I (4,SUC t), I (5,SUC t) and I (5,t) are not NONE **)
+   (`s.WB.WB_state_flag` by fs [Abbr `s`,enable_stg_def,agp32_ID_ID_write_enable_WB_state_flag] >>
+    `reg_data_vaild 5 s` by fs [Abbr `s`,reg_data_vaild_def] >>
+    `(agp32 fext fbits (SUC t)).R = (FUNPOW Next (THE (I' (5,t))) a).R` by cheat >> fs [] >>
+    `(agp32 fext fbits (SUC t)).ID.ID_addrB = (15 >< 10) i`
+      by (fs [Abbr `i`,Abbr `s`,is_sch_def] >>
+          METIS_TAC [agp32_Rel_ag32_ID_addr_correct,addrB_def]) >> fs [] >>
+    `enable_stg 5 (agp32 fext fbits t)`
+      by fs [enable_stg_def,agp32_ID_ID_write_enable_WB_state_flag] >>
+    `THE (I' (5,SUC t)) = THE (I' (5,t)) + 1` by METIS_TAC [WB_instr_index_t_SUC_t_enable] >>
+    `THE (I' (5,t)) = THE (I' (5,SUC t)) - 1` by fs [] >> fs [] >>
+    `(FUNPOW Next (THE (I' (5,SUC t)) − 1) a).R ((15 >< 10) i) =
+    (FUNPOW Next (THE (I' (5,SUC t))) a).R ((15 >< 10) i)`
+      by METIS_TAC [reg_adr_update_isa_not_change_data] >> fs [] >>
+    `THE (I' (4,SUC t)) = THE (I' (5,SUC t)) + 1`
+      by METIS_TAC [MEM_instr_index_with_WB_instr_plus_1] >>
+    `THE (I' (2,SUC t)) = THE (I' (4,SUC t)) + 1`
+      by METIS_TAC [EX_NONE_ID_instr_index_with_MEM_instr_plus_1] >> fs [] >>
+    `THE (I' (5,SUC t)) = THE (I' (4,SUC t)) - 1` by fs [] >>
+    METIS_TAC [reg_adr_update_isa_not_change_data]) >>
+  (** all are not NONE **)
+  `s.WB.WB_state_flag` by fs [Abbr `s`,enable_stg_def,agp32_ID_ID_write_enable_WB_state_flag] >>
+  `reg_data_vaild 5 s` by fs [Abbr `s`,reg_data_vaild_def] >>
+  `(agp32 fext fbits (SUC t)).R = (FUNPOW Next (THE (I' (5,t))) a).R` by cheat >> fs [] >>
+  `(agp32 fext fbits (SUC t)).ID.ID_addrB = (15 >< 10) i`
+    by (fs [Abbr `i`,Abbr `s`,is_sch_def] >>
+        METIS_TAC [agp32_Rel_ag32_ID_addr_correct,addrB_def]) >> fs [] >>
+  `enable_stg 5 (agp32 fext fbits t)`
+    by fs [enable_stg_def,agp32_ID_ID_write_enable_WB_state_flag] >>
+  `THE (I' (5,SUC t)) = THE (I' (5,t)) + 1` by METIS_TAC [WB_instr_index_t_SUC_t_enable] >>
+  `THE (I' (5,t)) = THE (I' (5,SUC t)) - 1` by fs [] >> fs [] >>
+  `(FUNPOW Next (THE (I' (5,SUC t)) − 1) a).R ((15 >< 10) i) =
+  (FUNPOW Next (THE (I' (5,SUC t))) a).R ((15 >< 10) i)`
+    by METIS_TAC [reg_adr_update_isa_not_change_data] >> fs [] >>
+  qpat_x_assum `THE (I' (5,SUC t)) = _` (fn thm => all_tac)  >>
+  `THE (I' (4,SUC t)) = THE (I' (5,SUC t)) + 1`
+    by METIS_TAC [MEM_instr_index_with_WB_instr_plus_1] >>
+  `THE (I' (5,SUC t)) = THE (I' (4,SUC t)) - 1` by fs [] >> fs [] >>
+  `(FUNPOW Next (THE (I' (4,SUC t)) − 1) a).R ((15 >< 10) i) =
+  (FUNPOW Next (THE (I' (4,SUC t))) a).R ((15 >< 10) i)`
+    by METIS_TAC [reg_adr_update_isa_not_change_data] >> fs [] >>
+  `THE (I' (3,SUC t)) = THE (I' (4,SUC t)) + 1`
+    by METIS_TAC [EX_instr_index_with_MEM_instr_plus_1] >>
+  `THE (I' (2,SUC t)) = THE (I' (3,SUC t)) + 1`
+    by METIS_TAC [ID_instr_index_with_EX_instr_plus_1] >> fs [] >>
+  `THE (I' (4,SUC t)) = THE (I' (3,SUC t)) - 1` by FULL_SIMP_TAC std_ss [] >>
+  METIS_TAC [reg_adr_update_isa_not_change_data]
+QED
+
+
+(** ID_read_dataW: when instrs in EX, MEM and WB do not change registers **)
+Theorem agp32_Rel_ag32_ID_read_dataW_no_write_before:
+  !fext fbits a t I.
+    is_sch I (agp32 fext fbits) a ==>
+    Rel I (fext t) (agp32 fext fbits (t-1)) (agp32 fext fbits t) a t ==>
+    enable_stg 2 (agp32 fext fbits t) ==>
+    I (2,SUC t) <> NONE ==>
+    ~reg_adr_update_isa (I (3,SUC t)) a (agp32 fext fbits (SUC t)).ID.ID_addrW ==>
+    ~reg_adr_update_isa (I (4,SUC t)) a (agp32 fext fbits (SUC t)).ID.ID_addrW ==>
+    ~reg_adr_update_isa (I (5,SUC t)) a (agp32 fext fbits (SUC t)).ID.ID_addrW ==>
+    (agp32 fext fbits (SUC t)).ID.ID_read_dataW = reg_dataW (FUNPOW Next (THE (I (2,SUC t)) − 1) a)
+Proof
+  rw [reg_dataW_def,addrW_def] >>
+  `(agp32 fext fbits (SUC t)).ID.ID_instr = instr (FUNPOW Next (THE (I' (2,SUC t)) − 1) a)`
+    by fs [is_sch_def,agp32_Rel_ag32_ID_instr_correct] >>
+  Q.ABBREV_TAC `s = agp32 fext fbits t` >>
+  Q.ABBREV_TAC `s' = procs [agp32_next_state; WB_pipeline; MEM_pipeline; EX_pipeline;
+                            REG_write; ID_pipeline; IF_PC_update; Acc_compute] (fext t) s s` >>
+  Q.ABBREV_TAC `s'' = procs [ForwardA; ForwardB; ForwardW; IF_instr_update;
+                             WB_update; ID_opc_func_update; ID_imm_update] (fext (SUC t)) s' s'` >>
+  `(agp32 fext fbits (SUC t)).ID.ID_read_dataW =
+  (ID_data_update (fext (SUC t)) s' s'').ID.ID_read_dataW`
+    by fs [Abbr `s`,Abbr `s'`,Abbr `s''`,agp32_ID_read_data_updated_by_ID_data_update] >>
+  fs [ID_data_update_def] >>
+  `s''.ID.ID_instr = (agp32 fext fbits (SUC t)).ID.ID_instr`
+    by fs [Abbr `s`,Abbr `s'`,Abbr `s''`,agp32_same_ID_instr_after_ID_imm_update] >> fs [] >>
+  qpat_abbrev_tac `i = instr _` >>
+  `s''.R = (agp32 fext fbits (SUC t)).R`
+    by fs [Abbr `s`,Abbr `s'`,Abbr `s''`,agp32_same_R_after_ID_imm_update] >> fs [] >>
+  Cases_on `I' (5,t) = NONE` >>
+  Cases_on `I' (5,SUC t) = NONE` >>
+  Cases_on `I' (4,SUC t) = NONE` >>
+  Cases_on `I' (3,SUC t) = NONE` >-
+   (** all NONE **)
+   (`(agp32 fext fbits (SUC t)).R = (FUNPOW Next (THE (I' (2,SUC t)) − 1) a).R`
+      by cheat >> fs []) >-
+   (** I (3,SUC t) is not NONE **)
+   (`(agp32 fext fbits (SUC t)).R = (FUNPOW Next (THE (I' (3,SUC t)) − 1) a).R`
+      by cheat >> fs [] >>
+    `(agp32 fext fbits (SUC t)).ID.ID_addrW = (30 >< 25) i`
+      by (fs [Abbr `i`,Abbr `s`,is_sch_def] >> METIS_TAC [agp32_Rel_ag32_ID_addr_correct,addrW_def]) >>
+    `THE (I' (2,SUC t)) = THE (I' (3,SUC t)) + 1`
+      by METIS_TAC [ID_instr_index_with_EX_instr_plus_1] >> fs [] >>
+    METIS_TAC [reg_adr_update_isa_not_change_data]) >-
+   (** I (4,SUC t) is not NONE **)
+   (`(agp32 fext fbits (SUC t)).R = (FUNPOW Next (THE (I' (4,SUC t)) − 1) a).R`
+      by cheat >> fs [] >>
+    `(agp32 fext fbits (SUC t)).ID.ID_addrW = (30 >< 25) i`
+      by (fs [Abbr `i`,Abbr `s`,is_sch_def] >> METIS_TAC [agp32_Rel_ag32_ID_addr_correct,addrW_def]) >>
+    fs [] >>
+    `(FUNPOW Next (THE (I' (4,SUC t)) − 1) a).R ((30 >< 25) i) =
+    (FUNPOW Next (THE (I' (4,SUC t))) a).R ((30 >< 25) i)`
+      by METIS_TAC [reg_adr_update_isa_not_change_data] >> fs [] >>
+    `THE (I' (2,SUC t)) = THE (I' (4,SUC t)) + 1`
+      by METIS_TAC [EX_NONE_ID_instr_index_with_MEM_instr_plus_1] >> fs []) >-
+   (** I (3,SUC t) and I (4,SUC t) are not NONE **)
+   (`(agp32 fext fbits (SUC t)).R = (FUNPOW Next (THE (I' (4,SUC t)) − 1) a).R`
+      by cheat >> fs [] >>
+    `(agp32 fext fbits (SUC t)).ID.ID_addrW = (30 >< 25) i`
+      by (fs [Abbr `i`,Abbr `s`,is_sch_def] >> METIS_TAC [agp32_Rel_ag32_ID_addr_correct,addrW_def]) >>
+    fs [] >>
+    `(FUNPOW Next (THE (I' (4,SUC t)) − 1) a).R ((30 >< 25) i) =
+    (FUNPOW Next (THE (I' (4,SUC t))) a).R ((30 >< 25) i)`
+      by METIS_TAC [reg_adr_update_isa_not_change_data] >> fs [] >>
+    `THE (I' (2,SUC t)) = THE (I' (3,SUC t)) + 1`
+      by METIS_TAC [ID_instr_index_with_EX_instr_plus_1] >> fs [] >>
+    `THE (I' (3,SUC t)) = THE (I' (4,SUC t)) + 1`
+      by METIS_TAC [EX_instr_index_with_MEM_instr_plus_1] >> fs [] >>
+    `THE (I' (4,SUC t)) = THE (I' (3,SUC t)) - 1` by fs [] >> fs [] >>
+    METIS_TAC [reg_adr_update_isa_not_change_data]) >-
+   (** I (5,SUC t) is not NONE **)
+   (`(agp32 fext fbits (SUC t)).R = (FUNPOW Next (THE (I' (5,SUC t)) − 1) a).R`
+      by cheat >> fs [] >>
+    `(agp32 fext fbits (SUC t)).ID.ID_addrW = (30 >< 25) i`
+      by (fs [Abbr `i`,Abbr `s`,is_sch_def] >>
+          METIS_TAC [agp32_Rel_ag32_ID_addr_correct,addrW_def]) >> fs [] >>
+    `(FUNPOW Next (THE (I' (5,SUC t)) − 1) a).R ((30 >< 25) i) =
+    (FUNPOW Next (THE (I' (5,SUC t))) a).R ((30 >< 25) i)`
+      by METIS_TAC [reg_adr_update_isa_not_change_data] >> fs [] >>
+    `THE (I' (2,SUC t)) = THE (I' (5,SUC t)) + 1`
+      by METIS_TAC [EX_MEM_NONE_ID_instr_index_with_WB_instr_plus_1] >> fs []) >-
+   (** I (3,SUC t) and I (5,SUC t) are not NONE **)
+   (`(agp32 fext fbits (SUC t)).R = (FUNPOW Next (THE (I' (5,SUC t)) − 1) a).R`
+      by cheat >> fs [] >>
+    `(agp32 fext fbits (SUC t)).ID.ID_addrW = (30 >< 25) i`
+      by (fs [Abbr `i`,Abbr `s`,is_sch_def] >>
+          METIS_TAC [agp32_Rel_ag32_ID_addr_correct,addrW_def]) >> fs [] >>
+    `(FUNPOW Next (THE (I' (5,SUC t)) − 1) a).R ((30 >< 25) i) =
+    (FUNPOW Next (THE (I' (5,SUC t))) a).R ((30 >< 25) i)`
+      by METIS_TAC [reg_adr_update_isa_not_change_data] >> fs [] >>
+    `THE (I' (3,SUC t)) = THE (I' (5,SUC t)) + 1`
+      by METIS_TAC [EX_instr_index_with_WB_instr_plus_1_MEM_NONE] >>
+    `THE (I' (2,SUC t)) = THE (I' (3,SUC t)) + 1`
+      by METIS_TAC [ID_instr_index_with_EX_instr_plus_1] >> fs [] >>
+    `THE (I' (5,SUC t)) = THE (I' (3,SUC t)) - 1` by fs [] >> fs [] >>
+    METIS_TAC [reg_adr_update_isa_not_change_data]) >-
+   (** I (4,SUC t) and I (5,SUC t) are not NONE **)
+   (`(agp32 fext fbits (SUC t)).R = (FUNPOW Next (THE (I' (5,SUC t)) − 1) a).R`
+      by cheat >> fs [] >>
+    `(agp32 fext fbits (SUC t)).ID.ID_addrW = (30 >< 25) i`
+      by (fs [Abbr `i`,Abbr `s`,is_sch_def] >>
+          METIS_TAC [agp32_Rel_ag32_ID_addr_correct,addrW_def]) >> fs [] >>
+    `(FUNPOW Next (THE (I' (5,SUC t)) − 1) a).R ((30 >< 25) i) =
+    (FUNPOW Next (THE (I' (5,SUC t))) a).R ((30 >< 25) i)`
+      by METIS_TAC [reg_adr_update_isa_not_change_data] >> fs [] >>
+    `THE (I' (4,SUC t)) = THE (I' (5,SUC t)) + 1`
+      by METIS_TAC [MEM_instr_index_with_WB_instr_plus_1] >>
+    `THE (I' (2,SUC t)) = THE (I' (4,SUC t)) + 1`
+      by METIS_TAC [EX_NONE_ID_instr_index_with_MEM_instr_plus_1] >> fs [] >>
+    `THE (I' (5,SUC t)) = THE (I' (4,SUC t)) - 1` by fs [] >> fs [] >>
+    METIS_TAC [reg_adr_update_isa_not_change_data]) >-
+   (** I (3,SUC t), I (4,SUC t) and I (5,SUC t) are not NONE **)
+   (`(agp32 fext fbits (SUC t)).R = (FUNPOW Next (THE (I' (5,SUC t)) − 1) a).R`
+      by cheat >> fs [] >>
+    `(agp32 fext fbits (SUC t)).ID.ID_addrW = (30 >< 25) i`
+      by (fs [Abbr `i`,Abbr `s`,is_sch_def] >>
+          METIS_TAC [agp32_Rel_ag32_ID_addr_correct,addrW_def]) >> fs [] >>
+    `(FUNPOW Next (THE (I' (5,SUC t)) − 1) a).R ((30 >< 25) i) =
+    (FUNPOW Next (THE (I' (5,SUC t))) a).R ((30 >< 25) i)`
+      by METIS_TAC [reg_adr_update_isa_not_change_data] >> fs [] >>
+    `THE (I' (4,SUC t)) = THE (I' (5,SUC t)) + 1`
+      by METIS_TAC [MEM_instr_index_with_WB_instr_plus_1] >>
+    `THE (I' (5,SUC t)) = THE (I' (4,SUC t)) - 1` by fs [] >> fs [] >>
+    `(FUNPOW Next (THE (I' (4,SUC t)) − 1) a).R ((30 >< 25) i) =
+    (FUNPOW Next (THE (I' (4,SUC t))) a).R ((30 >< 25) i)`
+      by METIS_TAC [reg_adr_update_isa_not_change_data] >> fs [] >>
+    `THE (I' (3,SUC t)) = THE (I' (4,SUC t)) + 1`
+      by METIS_TAC [EX_instr_index_with_MEM_instr_plus_1] >>
+    `THE (I' (2,SUC t)) = THE (I' (3,SUC t)) + 1`
+      by METIS_TAC [ID_instr_index_with_EX_instr_plus_1] >> fs [] >>
+    `THE (I' (4,SUC t)) = THE (I' (3,SUC t)) - 1` by FULL_SIMP_TAC std_ss [] >>
+    METIS_TAC [reg_adr_update_isa_not_change_data]) >-
+   (** I (5,t) is not NONE **)
+   (`s.WB.WB_state_flag` by fs [Abbr `s`,enable_stg_def,agp32_ID_ID_write_enable_WB_state_flag] >>
+    `reg_data_vaild 5 s` by fs [Abbr `s`,reg_data_vaild_def] >>
+    `(agp32 fext fbits (SUC t)).R = (FUNPOW Next (THE (I' (5,t))) a).R` by cheat >> fs [] >>
+    subgoal `I' (2,SUC t) = I' (1,t)` >-
+     (fs [is_sch_def,is_sch_decode_def,Abbr `s`] >>
+      Cases_on `isJump_isa_op (I' (2,t)) a \/ isJump_isa_op (I' (3,t)) a` >>
+      METIS_TAC []) >> fs [] >>
+    subgoal `I' (5,SUC t) = I' (4,t)` >-
+     (fs [is_sch_def,is_sch_writeback_def,is_sch_disable_def,Abbr `s`] >>
+      Cases_on `enable_stg 5 (agp32 fext fbits t)` >>
+      METIS_TAC []) >> fs [] >>
+    subgoal `I' (4,SUC t) = I' (3,t)` >-
+     (fs [is_sch_def,is_sch_memory_def,Abbr `s`] >>
+      `enable_stg 4 (agp32 fext fbits t)`
+        by fs [enable_stg_def,agp32_ID_ID_write_enable_MEM_state_flag] >>
+      Cases_on `isMemOp_hw_op (agp32 fext fbits t)` >>
+      fs [enable_stg_def] >>
+      METIS_TAC [MEM_stg_op_agp32_ID_EX_write_disable,
+                 agp32_ID_ID_write_enable_eq_ID_EX_write_enable]) >> fs [] >>
+    subgoal `I' (3,SUC t) = I' (2,t)` >-
+     (fs [is_sch_def,is_sch_execute_def,Abbr `s`] >>
+      `enable_stg 3 (agp32 fext fbits t)`
+        by fs [enable_stg_def,agp32_ID_ID_write_enable_eq_ID_EX_write_enable] >>
+      Cases_on `isJump_isa_op (I' (3,t)) a` >>
+      METIS_TAC [isJump_isa_op_not_none]) >> fs [] >>
+    `THE (I' (1,t)) = THE (I' (5,t)) + 1`
+      by METIS_TAC [ID_EX_MEM_NONE_IF_instr_index_with_WB_instr_plus_1] >> fs []) >-
+   (** I (3,SUC t) and I (5,t) are not NONE **)
+   (`s.WB.WB_state_flag` by fs [Abbr `s`,enable_stg_def,agp32_ID_ID_write_enable_WB_state_flag] >>
+    `reg_data_vaild 5 s` by fs [Abbr `s`,reg_data_vaild_def] >>
+    `(agp32 fext fbits (SUC t)).R = (FUNPOW Next (THE (I' (5,t))) a).R` by cheat >> fs [] >>
+    `(agp32 fext fbits (SUC t)).ID.ID_addrW = (30 >< 25) i`
+      by (fs [Abbr `i`,Abbr `s`,is_sch_def] >>
+          METIS_TAC [agp32_Rel_ag32_ID_addr_correct,addrW_def]) >> fs [] >>
+    subgoal `I' (2,SUC t) = I' (1,t)` >-
+     (fs [is_sch_def,is_sch_decode_def,Abbr `s`] >>
+      Cases_on `isJump_isa_op (I' (2,t)) a \/ isJump_isa_op (I' (3,t)) a` >>
+      METIS_TAC []) >> fs [] >>
+    subgoal `I' (5,SUC t) = I' (4,t)` >-
+     (fs [is_sch_def,is_sch_writeback_def,is_sch_disable_def,Abbr `s`] >>
+      Cases_on `enable_stg 5 (agp32 fext fbits t)` >>
+      METIS_TAC []) >> fs [] >>
+    subgoal `I' (4,SUC t) = I' (3,t)` >-
+     (fs [is_sch_def,is_sch_memory_def,Abbr `s`] >>
+      `enable_stg 4 (agp32 fext fbits t)`
+        by fs [enable_stg_def,agp32_ID_ID_write_enable_MEM_state_flag] >>
+      Cases_on `isMemOp_hw_op (agp32 fext fbits t)` >>
+      fs [enable_stg_def] >>
+      METIS_TAC [MEM_stg_op_agp32_ID_EX_write_disable,
+                 agp32_ID_ID_write_enable_eq_ID_EX_write_enable]) >> fs [] >>
+    subgoal `I' (3,SUC t) = I' (2,t)` >-
+     (fs [is_sch_def,is_sch_execute_def,Abbr `s`] >>
+      `enable_stg 3 (agp32 fext fbits t)`
+        by fs [enable_stg_def,agp32_ID_ID_write_enable_eq_ID_EX_write_enable] >>
+      Cases_on `isJump_isa_op (I' (3,t)) a` >>
+      METIS_TAC [isJump_isa_op_not_none]) >> fs [] >>
+    `THE (I' (2,t)) = THE (I' (5,t)) + 1`
+      by METIS_TAC [EX_MEM_NONE_ID_instr_index_with_WB_instr_plus_1] >>
+    `THE (I' (5,t)) = THE (I' (2,t)) - 1` by fs [] >>
+    `THE (I' (1,t)) = THE (I' (2,t)) + 1`
+      by METIS_TAC [IF_instr_index_with_ID_instr_plus_1] >> fs [] >>
+    METIS_TAC [reg_adr_update_isa_not_change_data]) >-
+   (** I (4,SUC t) and I (5,t) are not NONE **)
+   (`s.WB.WB_state_flag` by fs [Abbr `s`,enable_stg_def,agp32_ID_ID_write_enable_WB_state_flag] >>
+    `reg_data_vaild 5 s` by fs [Abbr `s`,reg_data_vaild_def] >>
+    `(agp32 fext fbits (SUC t)).R = (FUNPOW Next (THE (I' (5,t))) a).R` by cheat >> fs [] >>
+    `(agp32 fext fbits (SUC t)).ID.ID_addrW = (30 >< 25) i`
+      by (fs [Abbr `i`,Abbr `s`,is_sch_def] >>
+          METIS_TAC [agp32_Rel_ag32_ID_addr_correct,addrW_def]) >> fs [] >>
+    subgoal `THE (I' (4,SUC t)) = THE (I' (5,t)) + 1` >-
+     (`I' (5,SUC t) = I' (4,t)`
+        by (fs [is_sch_def,is_sch_writeback_def,is_sch_disable_def,Abbr `s`] >>
+            Cases_on `enable_stg 5 (agp32 fext fbits t)` >>
+            METIS_TAC []) >>
+      `I' (4,SUC t) = I' (3,t)`
+          by (fs [is_sch_def,is_sch_memory_def,Abbr `s`] >>
+              `enable_stg 4 (agp32 fext fbits t)`
+                by fs [enable_stg_def,agp32_ID_ID_write_enable_MEM_state_flag] >>
+              Cases_on `isMemOp_hw_op (agp32 fext fbits t)` >>
+              fs [enable_stg_def] >>
+              METIS_TAC [MEM_stg_op_agp32_ID_EX_write_disable,
+                         agp32_ID_ID_write_enable_eq_ID_EX_write_enable]) >> fs [] >>
+      METIS_TAC [EX_instr_index_with_WB_instr_plus_1_MEM_NONE]) >>
+    `THE (I' (5,t)) = THE (I' (4,SUC t)) - 1` by fs [] >> fs [] >>
+    `(FUNPOW Next (THE (I' (4,SUC t)) − 1) a).R ((30 >< 25) i) =
+    (FUNPOW Next (THE (I' (4,SUC t))) a).R ((30 >< 25) i)`
+      by METIS_TAC [reg_adr_update_isa_not_change_data] >> fs [] >>
+    `THE (I' (2,SUC t)) = THE (I' (4,SUC t)) + 1`
+      by METIS_TAC [EX_NONE_ID_instr_index_with_MEM_instr_plus_1] >> fs []) >-
+   (** I (3,SUC t), I (4,SUC t) and I (5,t) are not NONE **)
+   (`s.WB.WB_state_flag` by fs [Abbr `s`,enable_stg_def,agp32_ID_ID_write_enable_WB_state_flag] >>
+    `reg_data_vaild 5 s` by fs [Abbr `s`,reg_data_vaild_def] >>
+    `(agp32 fext fbits (SUC t)).R = (FUNPOW Next (THE (I' (5,t))) a).R` by cheat >> fs [] >>
+    `(agp32 fext fbits (SUC t)).ID.ID_addrW = (30 >< 25) i`
+      by (fs [Abbr `i`,Abbr `s`,is_sch_def] >>
+          METIS_TAC [agp32_Rel_ag32_ID_addr_correct,addrW_def]) >> fs [] >>
+    subgoal `THE (I' (4,SUC t)) = THE (I' (5,t)) + 1` >-
+     (`I' (5,SUC t) = I' (4,t)`
+        by (fs [is_sch_def,is_sch_writeback_def,is_sch_disable_def,Abbr `s`] >>
+            Cases_on `enable_stg 5 (agp32 fext fbits t)` >>
+            METIS_TAC []) >>
+      `I' (4,SUC t) = I' (3,t)`
+          by (fs [is_sch_def,is_sch_memory_def,Abbr `s`] >>
+              `enable_stg 4 (agp32 fext fbits t)`
+                by fs [enable_stg_def,agp32_ID_ID_write_enable_MEM_state_flag] >>
+              Cases_on `isMemOp_hw_op (agp32 fext fbits t)` >>
+              fs [enable_stg_def] >>
+              METIS_TAC [MEM_stg_op_agp32_ID_EX_write_disable,
+                         agp32_ID_ID_write_enable_eq_ID_EX_write_enable]) >> fs [] >>
+      METIS_TAC [EX_instr_index_with_WB_instr_plus_1_MEM_NONE]) >>
+    `THE (I' (5,t)) = THE (I' (4,SUC t)) - 1` by fs [] >> fs [] >>
+    `(FUNPOW Next (THE (I' (4,SUC t)) − 1) a).R ((30 >< 25) i) =
+    (FUNPOW Next (THE (I' (4,SUC t))) a).R ((30 >< 25) i)`
+      by METIS_TAC [reg_adr_update_isa_not_change_data] >> fs [] >>
+    `THE (I' (3,SUC t)) = THE (I' (4,SUC t)) + 1`
+      by METIS_TAC [EX_instr_index_with_MEM_instr_plus_1] >>
+    `THE (I' (2,SUC t)) = THE (I' (3,SUC t)) + 1`
+      by METIS_TAC [ID_instr_index_with_EX_instr_plus_1] >> fs [] >>
+    `THE (I' (4,SUC t)) = THE (I' (3,SUC t)) - 1` by FULL_SIMP_TAC std_ss [] >>
+    METIS_TAC [reg_adr_update_isa_not_change_data]) >-
+   (** I (5,SUC t) and I (5,t) are not NONE **)
+   (`s.WB.WB_state_flag` by fs [Abbr `s`,enable_stg_def,agp32_ID_ID_write_enable_WB_state_flag] >>
+    `reg_data_vaild 5 s` by fs [Abbr `s`,reg_data_vaild_def] >>
+    `(agp32 fext fbits (SUC t)).R = (FUNPOW Next (THE (I' (5,t))) a).R` by cheat >> fs [] >>
+    `(agp32 fext fbits (SUC t)).ID.ID_addrW = (30 >< 25) i`
+      by (fs [Abbr `i`,Abbr `s`,is_sch_def] >>
+          METIS_TAC [agp32_Rel_ag32_ID_addr_correct,addrW_def]) >> fs [] >>
+    `enable_stg 5 (agp32 fext fbits t)`
+      by fs [enable_stg_def,agp32_ID_ID_write_enable_WB_state_flag] >>
+    `THE (I' (5,SUC t)) = THE (I' (5,t)) + 1` by METIS_TAC [WB_instr_index_t_SUC_t_enable] >>
+    `THE (I' (5,t)) = THE (I' (5,SUC t)) - 1` by fs [] >> fs [] >>
+    `(FUNPOW Next (THE (I' (5,SUC t)) − 1) a).R ((30 >< 25) i) =
+    (FUNPOW Next (THE (I' (5,SUC t))) a).R ((30 >< 25) i)`
+      by METIS_TAC [reg_adr_update_isa_not_change_data] >> fs [] >>
+    `THE (I' (2,SUC t)) = THE (I' (5,SUC t)) + 1`
+      by METIS_TAC [EX_MEM_NONE_ID_instr_index_with_WB_instr_plus_1] >> fs []) >-
+   (** I (3,SUC t), I (5,SUC t) and I (5,t) are not NONE **)
+   (`s.WB.WB_state_flag` by fs [Abbr `s`,enable_stg_def,agp32_ID_ID_write_enable_WB_state_flag] >>
+    `reg_data_vaild 5 s` by fs [Abbr `s`,reg_data_vaild_def] >>
+    `(agp32 fext fbits (SUC t)).R = (FUNPOW Next (THE (I' (5,t))) a).R` by cheat >> fs [] >>
+    `(agp32 fext fbits (SUC t)).ID.ID_addrW = (30 >< 25) i`
+      by (fs [Abbr `i`,Abbr `s`,is_sch_def] >>
+          METIS_TAC [agp32_Rel_ag32_ID_addr_correct,addrW_def]) >> fs [] >>
+    `enable_stg 5 (agp32 fext fbits t)`
+      by fs [enable_stg_def,agp32_ID_ID_write_enable_WB_state_flag] >>
+    `THE (I' (5,SUC t)) = THE (I' (5,t)) + 1` by METIS_TAC [WB_instr_index_t_SUC_t_enable] >>
+    `THE (I' (5,t)) = THE (I' (5,SUC t)) - 1` by fs [] >> fs [] >>
+    `(FUNPOW Next (THE (I' (5,SUC t)) − 1) a).R ((30 >< 25) i) =
+    (FUNPOW Next (THE (I' (5,SUC t))) a).R ((30 >< 25) i)`
+      by METIS_TAC [reg_adr_update_isa_not_change_data] >> fs [] >>
+    `THE (I' (3,SUC t)) = THE (I' (5,SUC t)) + 1`
+      by METIS_TAC [EX_instr_index_with_WB_instr_plus_1_MEM_NONE] >>
+    `THE (I' (2,SUC t)) = THE (I' (3,SUC t)) + 1`
+      by METIS_TAC [ID_instr_index_with_EX_instr_plus_1] >> fs [] >>
+    `THE (I' (5,SUC t)) = THE (I' (3,SUC t)) - 1` by fs [] >>
+    METIS_TAC [reg_adr_update_isa_not_change_data]) >-
+   (** I (4,SUC t), I (5,SUC t) and I (5,t) are not NONE **)
+   (`s.WB.WB_state_flag` by fs [Abbr `s`,enable_stg_def,agp32_ID_ID_write_enable_WB_state_flag] >>
+    `reg_data_vaild 5 s` by fs [Abbr `s`,reg_data_vaild_def] >>
+    `(agp32 fext fbits (SUC t)).R = (FUNPOW Next (THE (I' (5,t))) a).R` by cheat >> fs [] >>
+    `(agp32 fext fbits (SUC t)).ID.ID_addrW = (30 >< 25) i`
+      by (fs [Abbr `i`,Abbr `s`,is_sch_def] >>
+          METIS_TAC [agp32_Rel_ag32_ID_addr_correct,addrW_def]) >> fs [] >>
+    `enable_stg 5 (agp32 fext fbits t)`
+      by fs [enable_stg_def,agp32_ID_ID_write_enable_WB_state_flag] >>
+    `THE (I' (5,SUC t)) = THE (I' (5,t)) + 1` by METIS_TAC [WB_instr_index_t_SUC_t_enable] >>
+    `THE (I' (5,t)) = THE (I' (5,SUC t)) - 1` by fs [] >> fs [] >>
+    `(FUNPOW Next (THE (I' (5,SUC t)) − 1) a).R ((30 >< 25) i) =
+    (FUNPOW Next (THE (I' (5,SUC t))) a).R ((30 >< 25) i)`
+      by METIS_TAC [reg_adr_update_isa_not_change_data] >> fs [] >>
+    `THE (I' (4,SUC t)) = THE (I' (5,SUC t)) + 1`
+      by METIS_TAC [MEM_instr_index_with_WB_instr_plus_1] >>
+    `THE (I' (2,SUC t)) = THE (I' (4,SUC t)) + 1`
+      by METIS_TAC [EX_NONE_ID_instr_index_with_MEM_instr_plus_1] >> fs [] >>
+    `THE (I' (5,SUC t)) = THE (I' (4,SUC t)) - 1` by fs [] >>
+    METIS_TAC [reg_adr_update_isa_not_change_data]) >>
+  (** all are not NONE **)
+  `s.WB.WB_state_flag` by fs [Abbr `s`,enable_stg_def,agp32_ID_ID_write_enable_WB_state_flag] >>
+  `reg_data_vaild 5 s` by fs [Abbr `s`,reg_data_vaild_def] >>
+  `(agp32 fext fbits (SUC t)).R = (FUNPOW Next (THE (I' (5,t))) a).R` by cheat >> fs [] >>
+  `(agp32 fext fbits (SUC t)).ID.ID_addrW = (30 >< 25) i`
+    by (fs [Abbr `i`,Abbr `s`,is_sch_def] >>
+        METIS_TAC [agp32_Rel_ag32_ID_addr_correct,addrW_def]) >> fs [] >>
+  `enable_stg 5 (agp32 fext fbits t)`
+    by fs [enable_stg_def,agp32_ID_ID_write_enable_WB_state_flag] >>
+  `THE (I' (5,SUC t)) = THE (I' (5,t)) + 1` by METIS_TAC [WB_instr_index_t_SUC_t_enable] >>
+  `THE (I' (5,t)) = THE (I' (5,SUC t)) - 1` by fs [] >> fs [] >>
+  `(FUNPOW Next (THE (I' (5,SUC t)) − 1) a).R ((30 >< 25) i) =
+  (FUNPOW Next (THE (I' (5,SUC t))) a).R ((30 >< 25) i)`
+    by METIS_TAC [reg_adr_update_isa_not_change_data] >> fs [] >>
+  qpat_x_assum `THE (I' (5,SUC t)) = _` (fn thm => all_tac)  >>
+  `THE (I' (4,SUC t)) = THE (I' (5,SUC t)) + 1`
+    by METIS_TAC [MEM_instr_index_with_WB_instr_plus_1] >>
+  `THE (I' (5,SUC t)) = THE (I' (4,SUC t)) - 1` by fs [] >> fs [] >>
+  `(FUNPOW Next (THE (I' (4,SUC t)) − 1) a).R ((30 >< 25) i) =
+  (FUNPOW Next (THE (I' (4,SUC t))) a).R ((30 >< 25) i)`
+    by METIS_TAC [reg_adr_update_isa_not_change_data] >> fs [] >>
+  `THE (I' (3,SUC t)) = THE (I' (4,SUC t)) + 1`
+    by METIS_TAC [EX_instr_index_with_MEM_instr_plus_1] >>
+  `THE (I' (2,SUC t)) = THE (I' (3,SUC t)) + 1`
+    by METIS_TAC [ID_instr_index_with_EX_instr_plus_1] >> fs [] >>
+  `THE (I' (4,SUC t)) = THE (I' (3,SUC t)) - 1` by FULL_SIMP_TAC std_ss [] >>
+  METIS_TAC [reg_adr_update_isa_not_change_data]
+QED
+
+
+(** ID_read_dataA_updated: when instrs in EX, MEM and WB do not change registers **)
+Theorem agp32_Rel_ag32_ID_read_dataA_updated_no_write_before:
+  !fext fbits a t I.
+    is_sch I (agp32 fext fbits) a ==>
+    Rel I (fext t) (agp32 fext fbits (t-1)) (agp32 fext fbits t) a t ==>
+    enable_stg 2 (agp32 fext fbits t) ==>
+    I (2,SUC t) <> NONE ==>
+    ~reg_adr_update_isa (I (3,SUC t)) a (agp32 fext fbits (SUC t)).ID.ID_addrA ==>
+    ~reg_adr_update_isa (I (4,SUC t)) a (agp32 fext fbits (SUC t)).ID.ID_addrA ==>
+    ~reg_adr_update_isa (I (5,SUC t)) a (agp32 fext fbits (SUC t)).ID.ID_addrA ==>
+    (agp32 fext fbits (SUC t)).ID.ID_read_dataA_updated =
+    reg_dataA (FUNPOW Next (THE (I (2,SUC t)) − 1) a)
+Proof
+  rw [] >>
+  `~(agp32 fext fbits (SUC t)).ID.ID_ForwardA`
+    by METIS_TAC [agp32_ID_ForwardA_flag_reg_adr_update_isa] >>
+  fs [agp32_ID_not_ForwardA_read_dataA_read_dataA_updated,agp32_Rel_ag32_ID_read_dataA_no_write_before]
+QED
+
+(** ID_read_dataB_updated: when instrs in EX, MEM and WB do not change registers **)
+Theorem agp32_Rel_ag32_ID_read_dataB_updated_no_write_before:
+  !fext fbits a t I.
+    is_sch I (agp32 fext fbits) a ==>
+    Rel I (fext t) (agp32 fext fbits (t-1)) (agp32 fext fbits t) a t ==>
+    enable_stg 2 (agp32 fext fbits t) ==>
+    I (2,SUC t) <> NONE ==>
+    ~reg_adr_update_isa (I (3,SUC t)) a (agp32 fext fbits (SUC t)).ID.ID_addrB ==>
+    ~reg_adr_update_isa (I (4,SUC t)) a (agp32 fext fbits (SUC t)).ID.ID_addrB ==>
+    ~reg_adr_update_isa (I (5,SUC t)) a (agp32 fext fbits (SUC t)).ID.ID_addrB ==>
+    (agp32 fext fbits (SUC t)).ID.ID_read_dataB_updated =
+    reg_dataB (FUNPOW Next (THE (I (2,SUC t)) − 1) a)
+Proof
+  rw [] >>
+  `~(agp32 fext fbits (SUC t)).ID.ID_ForwardB`
+    by METIS_TAC [agp32_ID_ForwardB_flag_reg_adr_update_isa] >>
+  fs [agp32_ID_not_ForwardB_read_dataB_read_dataB_updated,agp32_Rel_ag32_ID_read_dataB_no_write_before]
+QED
+
+(** ID_read_dataW_updated: when instrs in EX, MEM and WB do not change registers **)
+Theorem agp32_Rel_ag32_ID_read_dataW_updated_no_write_before:
+  !fext fbits a t I.
+    is_sch I (agp32 fext fbits) a ==>
+    Rel I (fext t) (agp32 fext fbits (t-1)) (agp32 fext fbits t) a t ==>
+    enable_stg 2 (agp32 fext fbits t) ==>
+    I (2,SUC t) <> NONE ==>
+    ~reg_adr_update_isa (I (3,SUC t)) a (agp32 fext fbits (SUC t)).ID.ID_addrW ==>
+    ~reg_adr_update_isa (I (4,SUC t)) a (agp32 fext fbits (SUC t)).ID.ID_addrW ==>
+    ~reg_adr_update_isa (I (5,SUC t)) a (agp32 fext fbits (SUC t)).ID.ID_addrW ==>
+    (agp32 fext fbits (SUC t)).ID.ID_read_dataW_updated =
+    reg_dataW (FUNPOW Next (THE (I (2,SUC t)) − 1) a)
+Proof
+  rw [] >>
+  `~(agp32 fext fbits (SUC t)).ID.ID_ForwardW`
+    by METIS_TAC [agp32_ID_ForwardW_flag_reg_adr_update_isa] >>
+  fs [agp32_ID_not_ForwardW_read_dataW_read_dataW_updated,agp32_Rel_ag32_ID_read_dataW_no_write_before]
+QED
+
+
+(** ID_dataA: when instrs in EX, MEM and WB do not change registers **)
+Theorem agp32_Rel_ag32_ID_dataA_no_write_before:
+  !fext fbits a t I.
+    is_sch I (agp32 fext fbits) a ==>
+    Rel I (fext t) (agp32 fext fbits (t-1)) (agp32 fext fbits t) a t ==>
+    enable_stg 2 (agp32 fext fbits t) ==>
+    I (2,SUC t) <> NONE ==>
+    ~(agp32 fext fbits (SUC t)).ID.ID_addrA_disable ==>
+    ~reg_adr_update_isa (I (3,SUC t)) a (agp32 fext fbits (SUC t)).ID.ID_addrA ==>
+    ~reg_adr_update_isa (I (4,SUC t)) a (agp32 fext fbits (SUC t)).ID.ID_addrA ==>
+    ~reg_adr_update_isa (I (5,SUC t)) a (agp32 fext fbits (SUC t)).ID.ID_addrA ==>
+    (agp32 fext fbits (SUC t)).ID.ID_dataA = dataA (FUNPOW Next (THE (I (2,SUC t)) − 1) a)
+Proof
+  rw [] >>
+  `~flagA (FUNPOW Next (THE (I' (2,SUC t)) − 1) a)`
+    by METIS_TAC [is_sch_def,agp32_Rel_ag32_ID_flag_correct] >>
+  rw [dataA_correct_rewrite_flag_imm_reg_data,v2w_single_0w] >>
+  fs [agp32_ID_addrA_enable_dataA_read_dataA_updated,
+      agp32_Rel_ag32_ID_read_dataA_updated_no_write_before]
+QED
+
+(** ID_dataB: when instrs in EX, MEM and WB do not change registers **)
+Theorem agp32_Rel_ag32_ID_dataB_no_write_before:
+  !fext fbits a t I.
+    is_sch I (agp32 fext fbits) a ==>
+    Rel I (fext t) (agp32 fext fbits (t-1)) (agp32 fext fbits t) a t ==>
+    enable_stg 2 (agp32 fext fbits t) ==>
+    I (2,SUC t) <> NONE ==>
+    ~(agp32 fext fbits (SUC t)).ID.ID_addrB_disable ==>
+    ~reg_adr_update_isa (I (3,SUC t)) a (agp32 fext fbits (SUC t)).ID.ID_addrB ==>
+    ~reg_adr_update_isa (I (4,SUC t)) a (agp32 fext fbits (SUC t)).ID.ID_addrB ==>
+    ~reg_adr_update_isa (I (5,SUC t)) a (agp32 fext fbits (SUC t)).ID.ID_addrB ==>
+    (agp32 fext fbits (SUC t)).ID.ID_dataB = dataB (FUNPOW Next (THE (I (2,SUC t)) − 1) a)
+Proof
+  rw [] >>
+  `~flagB (FUNPOW Next (THE (I' (2,SUC t)) − 1) a)`
+    by METIS_TAC [is_sch_def,agp32_Rel_ag32_ID_flag_correct] >>
+  rw [dataB_correct_rewrite_flag_imm_reg_data,v2w_single_0w] >>
+  fs [agp32_ID_addrB_enable_dataB_read_dataB_updated,
+      agp32_Rel_ag32_ID_read_dataB_updated_no_write_before]
+QED
+
+(** ID_dataW: when instrs in EX, MEM and WB do not change registers **)
+Theorem agp32_Rel_ag32_ID_dataW_no_write_before:
+  !fext fbits a t I.
+    is_sch I (agp32 fext fbits) a ==>
+    Rel I (fext t) (agp32 fext fbits (t-1)) (agp32 fext fbits t) a t ==>
+    enable_stg 2 (agp32 fext fbits t) ==>
+    I (2,SUC t) <> NONE ==>
+    ~(agp32 fext fbits (SUC t)).ID.ID_addrW_disable ==>
+    ~reg_adr_update_isa (I (3,SUC t)) a (agp32 fext fbits (SUC t)).ID.ID_addrW ==>
+    ~reg_adr_update_isa (I (4,SUC t)) a (agp32 fext fbits (SUC t)).ID.ID_addrW ==>
+    ~reg_adr_update_isa (I (5,SUC t)) a (agp32 fext fbits (SUC t)).ID.ID_addrW ==>
+    (agp32 fext fbits (SUC t)).ID.ID_dataW = dataW (FUNPOW Next (THE (I (2,SUC t)) − 1) a)
+Proof
+  rw [] >>
+  `~flagW (FUNPOW Next (THE (I' (2,SUC t)) − 1) a)`
+    by METIS_TAC [is_sch_def,agp32_Rel_ag32_ID_flag_correct] >>
+  rw [dataW_correct_rewrite_flag_imm_reg_data,v2w_single_0w] >>
+  fs [agp32_ID_addrW_enable_dataW_read_dataW_updated,
+      agp32_Rel_ag32_ID_read_dataW_updated_no_write_before]
+QED
+
+(** ID_read_dataA_updated: WB updates the reading data port **)
+Theorem agp32_Rel_ag32_ID_read_dataA_updated_only_WB_write_before:
+  !fext fbits a t I.
+    is_sch I (agp32 fext fbits) a ==>
+    Rel I (fext t) (agp32 fext fbits (t-1)) (agp32 fext fbits t) a t ==>
+    enable_stg 2 (agp32 fext fbits t) ==>
+    I (2,SUC t) <> NONE ==>
+    ~reg_adr_update_isa (I (3,SUC t)) a (agp32 fext fbits (SUC t)).ID.ID_addrA ==>
+    ~reg_adr_update_isa (I (4,SUC t)) a (agp32 fext fbits (SUC t)).ID.ID_addrA ==>
+    reg_adr_update_isa (I (5,SUC t)) a (agp32 fext fbits (SUC t)).ID.ID_addrA ==>
+    (agp32 fext fbits (SUC t)).ID.ID_read_dataA_updated =
+    reg_dataA (FUNPOW Next (THE (I (2,SUC t)) − 1) a)
+Proof
+  rw [] >>
+  `(agp32 fext fbits (SUC t)).ID.ID_ForwardA`
+    by METIS_TAC [agp32_ID_ForwardA_flag_reg_adr_update_isa] >>
   cheat
 QED
 
@@ -570,7 +1638,13 @@ Theorem agp32_Rel_ag32_ID_reg_data_Rel_correct:
                     (THE (I (2,SUC t))) (I (3,SUC t)) (I (4,SUC t)) (I (5,SUC t))
 Proof
   rw [ID_reg_data_Rel_def] >>
-  fs [agp32_Rel_ag32_ID_read_dataA_no_write_before] >>
+  fs [agp32_Rel_ag32_ID_read_dataA_no_write_before,agp32_Rel_ag32_ID_read_dataB_no_write_before,
+      agp32_Rel_ag32_ID_read_dataW_no_write_before,
+      agp32_Rel_ag32_ID_read_dataA_updated_no_write_before,
+      agp32_Rel_ag32_ID_read_dataB_updated_no_write_before,
+      agp32_Rel_ag32_ID_read_dataW_updated_no_write_before,
+      agp32_Rel_ag32_ID_dataA_no_write_before,agp32_Rel_ag32_ID_dataB_no_write_before,
+      agp32_Rel_ag32_ID_dataW_no_write_before] >>
   cheat
 QED
 
